@prefix geo: <http://www.opengis.net/ont/geosparql#> .
@prefix owl: <http://www.w3.org/2002/07/owl#> .
@prefix rdf: <http://www.w3.org/1999/02/22-rdf-syntax-ns#> .
@prefix xml: <http://www.w3.org/XML/1998/namespace> .
@prefix xsd: <http://www.w3.org/2001/XMLSchema#> .
@prefix coso: <http://sawgraph.spatialai.org/v1/contaminoso#> .
@prefix pfas: <http://sawgraph.spatialai.org/v1/pfas#> .
@prefix qudt: <https://qudt.org/schema/qudt/> .
@prefix rdfs: <http://www.w3.org/2000/01/rdf-schema#> .
@prefix skos: <http://www.w3.org/2004/02/skos/core#> .
@prefix sosa: <http://www.w3.org/ns/sosa/> .
@prefix time: <http://www.w3.org/2006/time#> .
@prefix terms: <http://purl.org/dc/terms/> .
@prefix prov-o: <http://www.w3.org/ns/prov#> .
@prefix schema: <http://schema.org/> .
@prefix me_egad: <http://sawgraph.spatialai.org/v1/me-egad#> .

<http://sawgraph.spatialai.org/v1/me-egad> rdf:type owl:Ontology ;
                                            terms:contributor "Shirly Stephen, Torsten Hahmann, Katrina Schweikart"@en ;
                                            terms:created "2024-02-28"@en ;
                                            terms:description "This ontology supports the SAWGraph project"@en ;
                                            terms:title "Ontology for EGAD's Sites and Sample Observations"@en ;
                                            owl:versionInfo "v 1.0"@en .

#################################################################
#    Annotation properties
#################################################################

###  http://purl.org/dc/terms/contributor
terms:contributor rdf:type owl:AnnotationProperty .


###  http://purl.org/dc/terms/created
terms:created rdf:type owl:AnnotationProperty .


###  http://purl.org/dc/terms/description
terms:description rdf:type owl:AnnotationProperty .


###  http://purl.org/dc/terms/title
terms:title rdf:type owl:AnnotationProperty .


###  http://schema.org/domainIncludes
schema:domainIncludes rdf:type owl:AnnotationProperty .


###  http://schema.org/rangeIncludes
schema:rangeIncludes rdf:type owl:AnnotationProperty .


###  http://www.w3.org/2004/02/skos/core#prefLabel
skos:prefLabel rdf:type owl:AnnotationProperty .


#################################################################
#    Object Properties
#################################################################

###  http://sawgraph.spatialai.org/v1/contaminoso#analysisMethod
coso:analysisMethod rdf:type owl:ObjectProperty ;
                    rdfs:subPropertyOf sosa:usedProcedure .


###  http://sawgraph.spatialai.org/v1/contaminoso#hasSamplePoint
coso:hasSamplePoint rdf:type owl:ObjectProperty .


###  http://sawgraph.spatialai.org/v1/contaminoso#observedAnalyte
coso:observedAnalyte rdf:type owl:ObjectProperty ;
                     rdfs:subPropertyOf sosa:observedProperty .


###  http://sawgraph.spatialai.org/v1/contaminoso#sampleCollectionMethod
coso:sampleCollectionMethod rdf:type owl:ObjectProperty ;
                            rdfs:subPropertyOf sosa:usedProcedure .


###  http://sawgraph.spatialai.org/v1/contaminoso#sampleMaterialType
coso:sampleMaterialType rdf:type owl:ObjectProperty .


###  http://sawgraph.spatialai.org/v1/me-egad#analyzedBy
me_egad:analyzedBy rdf:type owl:ObjectProperty ;
                   rdfs:comment "This property denotes the relation between the observation collection/observation and the lab that conducted the contaminant analysis." ;
                   rdfs:label "analyzed by" .


###  http://sawgraph.spatialai.org/v1/me-egad#observedAtSite
me_egad:observedAtSite rdf:type owl:ObjectProperty ;
                       rdfs:comment "This property denotes the relation between an EGAD observation collection and the corresponding EGAD site." ;
                       rdfs:label "observed at EGAD site" .


###  http://sawgraph.spatialai.org/v1/me-egad#sampleLocation
me_egad:sampleLocation rdf:type owl:ObjectProperty ;
                       rdfs:comment "egad sample collection location" .


###  http://sawgraph.spatialai.org/v1/me-egad#samplePointType
me_egad:samplePointType rdf:type owl:ObjectProperty ;
                        rdfs:comment "This property is used to denote the specific type of an EGAD sample point." ;
                        rdfs:label "egad sample point type" .


###  http://sawgraph.spatialai.org/v1/me-egad#siteType
me_egad:siteType rdf:type owl:ObjectProperty ;
                 rdfs:comment "This property is used to denote the specific type of an EGAD site." ;
                 rdfs:label "egad site type" .


###  http://www.opengis.net/ont/geosparql#hasGeometry
geo:hasGeometry rdf:type owl:ObjectProperty .


###  http://www.w3.org/2003/01/geo/wgs84_pos#hasGeometry
<http://www.w3.org/2003/01/geo/wgs84_pos#hasGeometry> rdf:type owl:ObjectProperty .


###  http://www.w3.org/ns/sosa/hasFeatureOfInterest
sosa:hasFeatureOfInterest rdf:type owl:ObjectProperty .


###  http://www.w3.org/ns/sosa/hasMember
sosa:hasMember rdf:type owl:ObjectProperty .


###  http://www.w3.org/ns/sosa/hasResult
sosa:hasResult rdf:type owl:ObjectProperty .


###  http://www.w3.org/ns/sosa/isSampleOf
sosa:isSampleOf rdf:type owl:ObjectProperty .


###  http://www.w3.org/ns/sosa/observedProperty
sosa:observedProperty rdf:type owl:ObjectProperty .


###  http://www.w3.org/ns/sosa/observedSample
sosa:observedSample rdf:type owl:ObjectProperty .


###  http://www.w3.org/ns/sosa/usedProcedure
sosa:usedProcedure rdf:type owl:ObjectProperty .


###  https://qudt.org/schema/qudt/hasUnit
qudt:hasUnit rdf:type owl:ObjectProperty .


#################################################################
#    Data properties
#################################################################

###  http://sawgraph.spatialai.org/v1/contaminoso#sampleCollectionTime
coso:sampleCollectionTime rdf:type owl:DatatypeProperty .


###  http://sawgraph.spatialai.org/v1/me-egad#sampleID
me_egad:sampleID rdf:type owl:DatatypeProperty ;
                 rdfs:label "egad sample ID" .


###  http://sawgraph.spatialai.org/v1/me-egad#samplePointNumber
me_egad:samplePointNumber rdf:type owl:DatatypeProperty ;
                          rdfs:label "egad sample point number" .


###  http://sawgraph.spatialai.org/v1/me-egad#samplePointWebName
me_egad:samplePointWebName rdf:type owl:DatatypeProperty ;
                           rdfs:label "egad sample point web name" .


###  http://www.w3.org/ns/sosa/resultTime
sosa:resultTime rdf:type owl:DatatypeProperty .


#################################################################
#    Classes
#################################################################

###  http://sawgraph.spatialai.org/v1/contaminoso#AnalysisMethod
coso:AnalysisMethod rdf:type owl:Class ;
                    rdfs:subClassOf sosa:Procedure .


###  http://sawgraph.spatialai.org/v1/contaminoso#Feature
coso:Feature rdf:type owl:Class ;
             rdfs:subClassOf geo:Feature .


###  http://sawgraph.spatialai.org/v1/contaminoso#MaterialSample
coso:MaterialSample rdf:type owl:Class ;
                    rdfs:subClassOf sosa:Sample .


###  http://sawgraph.spatialai.org/v1/contaminoso#SampleMaterial
coso:SampleMaterial rdf:type owl:Class .


###  http://sawgraph.spatialai.org/v1/contaminoso#SamplingMethod
coso:SamplingMethod rdf:type owl:Class ;
                    rdfs:subClassOf sosa:Procedure ;
                    rdfs:comment "Refers to the overall approach or technique used to collect samples from a particular environmental medium (e.g., air, water, soil). Grab sampling, passive sampling, and continuous sampling are examples of different sampling methods. Each method has its own set of protocols and considerations based on the nature of the environmental medium and the goals of the sampling activity." ;
                    rdfs:label "Sampling Method" .


###  http://sawgraph.spatialai.org/v1/me-egad#EGAD-ObservationCollection
me_egad:EGAD-ObservationCollection rdf:type owl:Class ;
                                   rdfs:subClassOf sosa:ObservationCollection ,
                                                   [ rdf:type owl:Restriction ;
                                                     owl:onProperty me_egad:analyzedBy ;
                                                     owl:someValuesFrom prov-o:Organization
                                                   ] ,
                                                   [ rdf:type owl:Restriction ;
                                                     owl:onProperty coso:analysisMethod ;
                                                     owl:allValuesFrom pfas:PFAS-AnalysisMethod
                                                   ] ,
                                                   [ rdf:type owl:Restriction ;
                                                     owl:onProperty me_egad:observedAtSite ;
                                                     owl:allValuesFrom me_egad:EGAD_Site
                                                   ] ,
                                                   [ rdf:type owl:Restriction ;
                                                     owl:onProperty sosa:hasFeatureOfInterest ;
                                                     owl:allValuesFrom me_egad:EGAD-SamplePoint
                                                   ] ,
                                                   [ rdf:type owl:Restriction ;
                                                     owl:onProperty sosa:hasMember ;
                                                     owl:allValuesFrom me_egad:EGAD-PFAS-Observation
                                                   ] ,
                                                   [ rdf:type owl:Restriction ;
                                                     owl:onProperty sosa:observedSample ;
                                                     owl:allValuesFrom me_egad:EGAD-Sample
                                                   ] ;
                                   rdfs:comment "This class denotes the collection of all PFAS type observations made against a specific sample collected from an EGAD sample point." ;
                                   rdfs:label "EGAD Observation Collection" .


###  http://sawgraph.spatialai.org/v1/me-egad#EGAD-PFAS-Concentration
me_egad:EGAD-PFAS-Concentration rdf:type owl:Class ;
                                rdfs:subClassOf pfas:PFAS-ContaminantMeasurement ;
                                rdfs:label "EGAD PFAS Concentration" .


###  http://sawgraph.spatialai.org/v1/me-egad#EGAD-PFAS-MDL
me_egad:EGAD-PFAS-MDL rdf:type owl:Class ;
                      rdfs:subClassOf pfas:PFAS-ContaminantMeasurement ;
                      rdfs:label "EGAD PFAS Method Detection Limit (MDL)" .


###  http://sawgraph.spatialai.org/v1/me-egad#EGAD-PFAS-Observation
me_egad:EGAD-PFAS-Observation rdf:type owl:Class ;
                              rdfs:subClassOf pfas:PFAS-ContaminantObservation ,
                                              [ rdf:type owl:Restriction ;
                                                owl:onProperty sosa:hasResult ;
                                                owl:someValuesFrom me_egad:EGAD-PFAS-Concentration
                                              ] ,
                                              [ rdf:type owl:Restriction ;
                                                owl:onProperty sosa:hasResult ;
                                                owl:someValuesFrom me_egad:EGAD-PFAS-MDL
                                              ] ,
                                              [ rdf:type owl:Restriction ;
                                                owl:onProperty sosa:hasResult ;
                                                owl:someValuesFrom me_egad:EGAD-PFAS-QL
                                              ] ,
                                              [ rdf:type owl:Restriction ;
                                                owl:onProperty coso:observedAnalyte ;
                                                owl:allValuesFrom pfas:PFAS
                                              ] ;
                              rdfs:label "EGAD PFAS Observation" .


###  http://sawgraph.spatialai.org/v1/me-egad#EGAD-PFAS-QL
me_egad:EGAD-PFAS-QL rdf:type owl:Class ;
                     rdfs:subClassOf pfas:PFAS-ContaminantMeasurement ;
                     rdfs:label "EGAD PFAS Quantitation Limit (QL)" .


###  http://sawgraph.spatialai.org/v1/me-egad#EGAD-Sample
me_egad:EGAD-Sample rdf:type owl:Class ;
                    rdfs:subClassOf coso:MaterialSample ,
                                    [ rdf:type owl:Restriction ;
                                      owl:onProperty me_egad:sampleLocation ;
                                      owl:someValuesFrom me_egad:EGAD-SampleLocation
                                    ] ,
                                    [ rdf:type owl:Restriction ;
                                      owl:onProperty coso:sampleCollectionMethod ;
                                      owl:allValuesFrom me_egad:EGAD-SampleCollectionMethod
                                    ] ,
                                    [ rdf:type owl:Restriction ;
                                      owl:onProperty coso:sampleMaterialType ;
                                      owl:allValuesFrom me_egad:EGAD-SampleMaterialType
                                    ] .


###  http://sawgraph.spatialai.org/v1/me-egad#EGAD-SampleCollectionLocation
me_egad:EGAD-SampleCollectionLocation rdf:type owl:Class ;
                                      rdfs:label "EGAD Sample Collection Method" .


###  http://sawgraph.spatialai.org/v1/me-egad#EGAD-SampleCollectionMethod
me_egad:EGAD-SampleCollectionMethod rdf:type owl:Class ;
                                    rdfs:subClassOf coso:SamplingMethod .


###  http://sawgraph.spatialai.org/v1/me-egad#EGAD-SampleLocation
me_egad:EGAD-SampleLocation rdf:type owl:Class ;
                            rdfs:label "EGAD Sample Collection Location" .


###  http://sawgraph.spatialai.org/v1/me-egad#EGAD-SampleMaterialType
me_egad:EGAD-SampleMaterialType rdf:type owl:Class ;
                                rdfs:subClassOf coso:SampleMaterial .


###  http://sawgraph.spatialai.org/v1/me-egad#EGAD-SamplePoint
me_egad:EGAD-SamplePoint rdf:type owl:Class ;
                         rdfs:subClassOf coso:Feature ,
                                         sosa:FeatureOfInterest ,
                                         [ rdf:type owl:Restriction ;
                                           owl:onProperty me_egad:samplePointType ;
                                           owl:allValuesFrom me_egad:EGAD-SamplePointType
                                         ] ;
                         rdfs:comment "EGAD Sample Point class denotes the \"location\" where a DEP sample is collected." ;
                         rdfs:label "EGAD Sample Point" .


###  http://sawgraph.spatialai.org/v1/me-egad#EGAD-SamplePointType
me_egad:EGAD-SamplePointType rdf:type owl:Class ;
                             rdfs:label "EGAD Sample Point Type" .


###  http://sawgraph.spatialai.org/v1/me-egad#EGAD-SiteType
me_egad:EGAD-SiteType rdf:type owl:Class ;
                      rdfs:comment """EGAD Site Type class denotes types of all current Maine DEP's sites (alongside their definitions) including sites with land use activities which are potential and/or actual sources of contamination and sites where biological, groundwater, and surface water sampling is conducted.

Source: https://www.maine.gov/dep/maps-data/egad/documents/EGAD_Lookup_Tables.xlsx""" ;
                      rdfs:label "EGAD Site Type" .


###  http://sawgraph.spatialai.org/v1/me-egad#EGAD_Site
me_egad:EGAD_Site rdf:type owl:Class ;
                  rdfs:subClassOf coso:Feature ,
                                  [ rdf:type owl:Restriction ;
                                    owl:onProperty coso:hasSamplePoint ;
                                    owl:someValuesFrom me_egad:EGAD-SamplePoint
                                  ] ,
                                  [ rdf:type owl:Restriction ;
                                    owl:onProperty me_egad:siteType ;
                                    owl:allValuesFrom me_egad:EGAD-SiteType
                                  ] ,
                                  [ rdf:type owl:Restriction ;
                                    owl:onProperty <http://www.w3.org/2003/01/geo/wgs84_pos#hasGeometry> ;
                                    owl:allValuesFrom geo:Geometry
                                  ] ;
                  rdfs:comment """EGAD Site class denotes locations which are a potential and/or actual sources of contamination. Some of these are sites where groundwater, biological, and surface water sampling is or has been conducted.

See me_egad:EGAD-SiteType for different site types.""" ;
                  rdfs:label "EGAD Site" .


###  http://sawgraph.spatialai.org/v1/pfas#PFAS
pfas:PFAS rdf:type owl:Class ;
          rdfs:subClassOf sosa:ObservedProperty .


###  http://sawgraph.spatialai.org/v1/pfas#PFAS-AnalysisMethod
pfas:PFAS-AnalysisMethod rdf:type owl:Class ;
                         rdfs:subClassOf coso:AnalysisMethod .


###  http://sawgraph.spatialai.org/v1/pfas#PFAS-ContaminantMeasurement
pfas:PFAS-ContaminantMeasurement rdf:type owl:Class ;
                                 rdfs:subClassOf sosa:Result .


###  http://sawgraph.spatialai.org/v1/pfas#PFAS-ContaminantObservation
pfas:PFAS-ContaminantObservation rdf:type owl:Class ;
                                 rdfs:subClassOf sosa:Observation .


###  http://www.opengis.net/ont/geosparql#Feature
geo:Feature rdf:type owl:Class .


###  http://www.opengis.net/ont/geosparql#Geometry
geo:Geometry rdf:type owl:Class .


###  http://www.w3.org/2006/time#TemporalEntity
time:TemporalEntity rdf:type owl:Class .


###  http://www.w3.org/ns/prov#Organization
prov-o:Organization rdf:type owl:Class .


###  http://www.w3.org/ns/sosa/FeatureOfInterest
sosa:FeatureOfInterest rdf:type owl:Class .


###  http://www.w3.org/ns/sosa/Observation
sosa:Observation rdf:type owl:Class .


###  http://www.w3.org/ns/sosa/ObservationCollection
sosa:ObservationCollection rdf:type owl:Class .


###  http://www.w3.org/ns/sosa/ObservedProperty
sosa:ObservedProperty rdf:type owl:Class .


###  http://www.w3.org/ns/sosa/Procedure
sosa:Procedure rdf:type owl:Class .


###  http://www.w3.org/ns/sosa/Result
sosa:Result rdf:type owl:Class .


###  http://www.w3.org/ns/sosa/Sample
sosa:Sample rdf:type owl:Class ;
            rdfs:label "Sample" .


###  https://qudt.org/schema/qudt/QuantityValue
qudt:QuantityValue rdf:type owl:Class .


###  https://qudt.org/schema/qudt/Unit
qudt:Unit rdf:type owl:Class .


#################################################################
#    Individuals
#################################################################

###  http://sawgraph.spatialai.org/v1/me-egad#sampleCollectionLocation.b
me_egad:sampleCollectionLocation.b rdf:type owl:NamedIndividual ,
                                            me_egad:EGAD-SampleLocation ;
                                   rdfs:label "BOAT" .


###  http://sawgraph.spatialai.org/v1/me-egad#sampleCollectionMethod.al
me_egad:sampleCollectionMethod.al rdf:type owl:NamedIndividual ,
                                           me_egad:EGAD-SampleCollectionLocation ;
                                  rdfs:label "DRILL RIG AIR LIFT" .


###  http://sawgraph.spatialai.org/v1/me-egad#sampleCollectionMethod.ang
me_egad:sampleCollectionMethod.ang rdf:type owl:NamedIndividual ,
                                            me_egad:EGAD-SampleCollectionLocation ;
                                   rdfs:label "ANGLING" .


###  http://sawgraph.spatialai.org/v1/me-egad#sampleCollectionMethod.ari
me_egad:sampleCollectionMethod.ari rdf:type owl:NamedIndividual ,
                                            me_egad:EGAD-SampleCollectionLocation ;
                                   rdfs:label "ARI SAMPLER" .


###  http://sawgraph.spatialai.org/v1/me-egad#sampleCollectionMethod.brs
me_egad:sampleCollectionMethod.brs rdf:type owl:NamedIndividual ,
                                            me_egad:EGAD-SampleCollectionLocation ;
                                   rdfs:label "BRUSH SCRAPINGS" .


###  http://sawgraph.spatialai.org/v1/me-egad#sampleCollectionMethod.bs
me_egad:sampleCollectionMethod.bs rdf:type owl:NamedIndividual ,
                                           me_egad:EGAD-SampleCollectionLocation ;
                                  rdfs:label "BAILED SAMPLE" .


###  http://sawgraph.spatialai.org/v1/me-egad#sampleCollectionMethod.bsp
me_egad:sampleCollectionMethod.bsp rdf:type owl:NamedIndividual ,
                                            me_egad:EGAD-SampleCollectionLocation ;
                                   rdfs:label "BRICK SCRAPINGS" .


###  http://sawgraph.spatialai.org/v1/me-egad#sampleCollectionMethod.c
me_egad:sampleCollectionMethod.c rdf:type owl:NamedIndividual ,
                                          me_egad:EGAD-SampleCollectionLocation ;
                                 rdfs:label "CONE" .


###  http://sawgraph.spatialai.org/v1/me-egad#sampleCollectionMethod.cg
me_egad:sampleCollectionMethod.cg rdf:type owl:NamedIndividual ,
                                           me_egad:EGAD-SampleCollectionLocation ;
                                  rdfs:label "CAGE" .


###  http://sawgraph.spatialai.org/v1/me-egad#sampleCollectionMethod.cle
me_egad:sampleCollectionMethod.cle rdf:type owl:NamedIndividual ,
                                            me_egad:EGAD-SampleCollectionLocation ;
                                   rdfs:label "CAPTURE-LETHAL" .


###  http://sawgraph.spatialai.org/v1/me-egad#sampleCollectionMethod.cli
me_egad:sampleCollectionMethod.cli rdf:type owl:NamedIndividual ,
                                            me_egad:EGAD-SampleCollectionLocation ;
                                   rdfs:label "CAPTURE-LIVE" .


###  http://sawgraph.spatialai.org/v1/me-egad#sampleCollectionMethod.cm
me_egad:sampleCollectionMethod.cm rdf:type owl:NamedIndividual ,
                                           me_egad:EGAD-SampleCollectionLocation ;
                                  rdfs:label "COMPASS" .


###  http://sawgraph.spatialai.org/v1/me-egad#sampleCollectionMethod.cmd
me_egad:sampleCollectionMethod.cmd rdf:type owl:NamedIndividual ,
                                            me_egad:EGAD-SampleCollectionLocation ;
                                   rdfs:label "CONTINUOUS MONITORING DEVICE" .


###  http://sawgraph.spatialai.org/v1/me-egad#sampleCollectionMethod.co
me_egad:sampleCollectionMethod.co rdf:type owl:NamedIndividual ,
                                           me_egad:EGAD-SampleCollectionLocation ;
                                  rdfs:label "CORE SAMPLE" .


###  http://sawgraph.spatialai.org/v1/me-egad#sampleCollectionMethod.crb
me_egad:sampleCollectionMethod.crb rdf:type owl:NamedIndividual ,
                                            me_egad:EGAD-SampleCollectionLocation ;
                                   rdfs:label "CONTROLLED RELEASE BAILER" .


###  http://sawgraph.spatialai.org/v1/me-egad#sampleCollectionMethod.cs
me_egad:sampleCollectionMethod.cs rdf:type owl:NamedIndividual ,
                                           me_egad:EGAD-SampleCollectionLocation ;
                                  rdfs:label "COMPOSITE SAMPLE" .


###  http://sawgraph.spatialai.org/v1/me-egad#sampleCollectionMethod.ct
me_egad:sampleCollectionMethod.ct rdf:type owl:NamedIndividual ,
                                           me_egad:EGAD-SampleCollectionLocation ;
                                  rdfs:label "CHARCOAL TUBE" .


###  http://sawgraph.spatialai.org/v1/me-egad#sampleCollectionMethod.dbs
me_egad:sampleCollectionMethod.dbs rdf:type owl:NamedIndividual ,
                                            me_egad:EGAD-SampleCollectionLocation ;
                                   rdfs:label "DEP BACTERIA SAMPLER" .


###  http://sawgraph.spatialai.org/v1/me-egad#sampleCollectionMethod.dfns
me_egad:sampleCollectionMethod.dfns rdf:type owl:NamedIndividual ,
                                             me_egad:EGAD-SampleCollectionLocation ;
                                    rdfs:label "D FRAME NET SWEEP" .


###  http://sawgraph.spatialai.org/v1/me-egad#sampleCollectionMethod.dl
me_egad:sampleCollectionMethod.dl rdf:type owl:NamedIndividual ,
                                           me_egad:EGAD-SampleCollectionLocation ;
                                  rdfs:label "WATER LEVEL DATA LOGGER" .


###  http://sawgraph.spatialai.org/v1/me-egad#sampleCollectionMethod.dm
me_egad:sampleCollectionMethod.dm rdf:type owl:NamedIndividual ,
                                           me_egad:EGAD-SampleCollectionLocation ;
                                  rdfs:label "DIRECT MEASURE" .


###  http://sawgraph.spatialai.org/v1/me-egad#sampleCollectionMethod.dn
me_egad:sampleCollectionMethod.dn rdf:type owl:NamedIndividual ,
                                           me_egad:EGAD-SampleCollectionLocation ;
                                  rdfs:label "DIPNET" .


###  http://sawgraph.spatialai.org/v1/me-egad#sampleCollectionMethod.dp
me_egad:sampleCollectionMethod.dp rdf:type owl:NamedIndividual ,
                                           me_egad:EGAD-SampleCollectionLocation ;
                                  rdfs:label "DIRECT PUSH SAMPLE" .


###  http://sawgraph.spatialai.org/v1/me-egad#sampleCollectionMethod.dpb
me_egad:sampleCollectionMethod.dpb rdf:type owl:NamedIndividual ,
                                            me_egad:EGAD-SampleCollectionLocation ;
                                   rdfs:label "DIRECT PUSH-BAILED SAMPLE" .


###  http://sawgraph.spatialai.org/v1/me-egad#sampleCollectionMethod.dpl
me_egad:sampleCollectionMethod.dpl rdf:type owl:NamedIndividual ,
                                            me_egad:EGAD-SampleCollectionLocation ;
                                   rdfs:label "DIRECT PUSH-LOW FLOW SAMPLE" .


###  http://sawgraph.spatialai.org/v1/me-egad#sampleCollectionMethod.dpn
me_egad:sampleCollectionMethod.dpn rdf:type owl:NamedIndividual ,
                                            me_egad:EGAD-SampleCollectionLocation ;
                                   rdfs:label "DIRECT PUSH-NO PURGE SAMPLE" .


###  http://sawgraph.spatialai.org/v1/me-egad#sampleCollectionMethod.dpp
me_egad:sampleCollectionMethod.dpp rdf:type owl:NamedIndividual ,
                                            me_egad:EGAD-SampleCollectionLocation ;
                                   rdfs:label "DIRECT PROBE/PEN (IN-SITU)" .


###  http://sawgraph.spatialai.org/v1/me-egad#sampleCollectionMethod.ds
me_egad:sampleCollectionMethod.ds rdf:type owl:NamedIndividual ,
                                           me_egad:EGAD-SampleCollectionLocation ;
                                  rdfs:label "DIFFUSION SAMPLE" .


###  http://sawgraph.spatialai.org/v1/me-egad#sampleCollectionMethod.dsd
me_egad:sampleCollectionMethod.dsd rdf:type owl:NamedIndividual ,
                                            me_egad:EGAD-SampleCollectionLocation ;
                                   rdfs:label "DEEP DIFFUSION SAMPLE" .


###  http://sawgraph.spatialai.org/v1/me-egad#sampleCollectionMethod.dsm
me_egad:sampleCollectionMethod.dsm rdf:type owl:NamedIndividual ,
                                            me_egad:EGAD-SampleCollectionLocation ;
                                   rdfs:label "MID DIFFUSION SAMPLE" .


###  http://sawgraph.spatialai.org/v1/me-egad#sampleCollectionMethod.dss
me_egad:sampleCollectionMethod.dss rdf:type owl:NamedIndividual ,
                                            me_egad:EGAD-SampleCollectionLocation ;
                                   rdfs:label "SHALLOW DIFFUSION SAMPLE" .


###  http://sawgraph.spatialai.org/v1/me-egad#sampleCollectionMethod.ef
me_egad:sampleCollectionMethod.ef rdf:type owl:NamedIndividual ,
                                           me_egad:EGAD-SampleCollectionLocation ;
                                  rdfs:label "ELECTROFISHING" .


###  http://sawgraph.spatialai.org/v1/me-egad#sampleCollectionMethod.ek
me_egad:sampleCollectionMethod.ek rdf:type owl:NamedIndividual ,
                                           me_egad:EGAD-SampleCollectionLocation ;
                                  rdfs:label "ECKMAN" .


###  http://sawgraph.spatialai.org/v1/me-egad#sampleCollectionMethod.ep
me_egad:sampleCollectionMethod.ep rdf:type owl:NamedIndividual ,
                                           me_egad:EGAD-SampleCollectionLocation ;
                                  rdfs:label "EEL POT" .


###  http://sawgraph.spatialai.org/v1/me-egad#sampleCollectionMethod.epgs
me_egad:sampleCollectionMethod.epgs rdf:type owl:NamedIndividual ,
                                             me_egad:EGAD-SampleCollectionLocation ;
                                    rdfs:label "EXTENSION POLE (GRAB)" .


###  http://sawgraph.spatialai.org/v1/me-egad#sampleCollectionMethod.epis
me_egad:sampleCollectionMethod.epis rdf:type owl:NamedIndividual ,
                                             me_egad:EGAD-SampleCollectionLocation ;
                                    rdfs:label "EXTENSION POLE (IN-SITU)" .


###  http://sawgraph.spatialai.org/v1/me-egad#sampleCollectionMethod.exp
me_egad:sampleCollectionMethod.exp rdf:type owl:NamedIndividual ,
                                            me_egad:EGAD-SampleCollectionLocation ;
                                   rdfs:label "EXPERIMENTAL" .


###  http://sawgraph.spatialai.org/v1/me-egad#sampleCollectionMethod.fm
me_egad:sampleCollectionMethod.fm rdf:type owl:NamedIndividual ,
                                           me_egad:EGAD-SampleCollectionLocation ;
                                  rdfs:label "FLOW METER" .


###  http://sawgraph.spatialai.org/v1/me-egad#sampleCollectionMethod.fn
me_egad:sampleCollectionMethod.fn rdf:type owl:NamedIndividual ,
                                           me_egad:EGAD-SampleCollectionLocation ;
                                  rdfs:label "FYKE NET" .


###  http://sawgraph.spatialai.org/v1/me-egad#sampleCollectionMethod.gn
me_egad:sampleCollectionMethod.gn rdf:type owl:NamedIndividual ,
                                           me_egad:EGAD-SampleCollectionLocation ;
                                  rdfs:label "GILL NET" .


###  http://sawgraph.spatialai.org/v1/me-egad#sampleCollectionMethod.gs
me_egad:sampleCollectionMethod.gs rdf:type owl:NamedIndividual ,
                                           me_egad:EGAD-SampleCollectionLocation ;
                                  rdfs:label "GRAB SAMPLE" .


###  http://sawgraph.spatialai.org/v1/me-egad#sampleCollectionMethod.gsfd
me_egad:sampleCollectionMethod.gsfd rdf:type owl:NamedIndividual ,
                                             me_egad:EGAD-SampleCollectionLocation ;
                                    rdfs:label "GRAB SAMPLE- FIRST DRAW" .


###  http://sawgraph.spatialai.org/v1/me-egad#sampleCollectionMethod.ha
me_egad:sampleCollectionMethod.ha rdf:type owl:NamedIndividual ,
                                           me_egad:EGAD-SampleCollectionLocation ;
                                  rdfs:label "HAND AUGER" .


###  http://sawgraph.spatialai.org/v1/me-egad#sampleCollectionMethod.hd
me_egad:sampleCollectionMethod.hd rdf:type owl:NamedIndividual ,
                                           me_egad:EGAD-SampleCollectionLocation ;
                                  rdfs:label "HESTER-DENDY" .


###  http://sawgraph.spatialai.org/v1/me-egad#sampleCollectionMethod.hnp
me_egad:sampleCollectionMethod.hnp rdf:type owl:NamedIndividual ,
                                            me_egad:EGAD-SampleCollectionLocation ;
                                   rdfs:label "HAND PUMP" .


###  http://sawgraph.spatialai.org/v1/me-egad#sampleCollectionMethod.hp
me_egad:sampleCollectionMethod.hp rdf:type owl:NamedIndividual ,
                                           me_egad:EGAD-SampleCollectionLocation ;
                                  rdfs:label "HAND-PICKED" .


###  http://sawgraph.spatialai.org/v1/me-egad#sampleCollectionMethod.hs
me_egad:sampleCollectionMethod.hs rdf:type owl:NamedIndividual ,
                                           me_egad:EGAD-SampleCollectionLocation ;
                                  rdfs:label "HIGH ACCURACY SURVEY" .


###  http://sawgraph.spatialai.org/v1/me-egad#sampleCollectionMethod.ip
me_egad:sampleCollectionMethod.ip rdf:type owl:NamedIndividual ,
                                           me_egad:EGAD-SampleCollectionLocation ;
                                  rdfs:label "INTERFACE PROBE" .


###  http://sawgraph.spatialai.org/v1/me-egad#sampleCollectionMethod.is
me_egad:sampleCollectionMethod.is rdf:type owl:NamedIndividual ,
                                           me_egad:EGAD-SampleCollectionLocation ;
                                  rdfs:label "IN-SITU" .


###  http://sawgraph.spatialai.org/v1/me-egad#sampleCollectionMethod.isco
me_egad:sampleCollectionMethod.isco rdf:type owl:NamedIndividual ,
                                             me_egad:EGAD-SampleCollectionLocation ;
                                    rdfs:label "ISCO AUTOMATED SAMPLER" .


###  http://sawgraph.spatialai.org/v1/me-egad#sampleCollectionMethod.iss
me_egad:sampleCollectionMethod.iss rdf:type owl:NamedIndividual ,
                                            me_egad:EGAD-SampleCollectionLocation ;
                                   rdfs:label "INCREMENTAL SOIL SAMPLE" .


###  http://sawgraph.spatialai.org/v1/me-egad#sampleCollectionMethod.kem
me_egad:sampleCollectionMethod.kem rdf:type owl:NamedIndividual ,
                                            me_egad:EGAD-SampleCollectionLocation ;
                                   rdfs:label "KEMMERER" .


###  http://sawgraph.spatialai.org/v1/me-egad#sampleCollectionMethod.kq
me_egad:sampleCollectionMethod.kq rdf:type owl:NamedIndividual ,
                                           me_egad:EGAD-SampleCollectionLocation ;
                                  rdfs:label "KICK-QUALITATIVE" .


###  http://sawgraph.spatialai.org/v1/me-egad#sampleCollectionMethod.lfgf
me_egad:sampleCollectionMethod.lfgf rdf:type owl:NamedIndividual ,
                                             me_egad:EGAD-SampleCollectionLocation ;
                                    rdfs:label "LANDFILL GAS FIELD INSTRUMENT" .


###  http://sawgraph.spatialai.org/v1/me-egad#sampleCollectionMethod.lfgs
me_egad:sampleCollectionMethod.lfgs rdf:type owl:NamedIndividual ,
                                             me_egad:EGAD-SampleCollectionLocation ;
                                    rdfs:label "LANDFILL GAS STATIONARY INSTRUMENT" .


###  http://sawgraph.spatialai.org/v1/me-egad#sampleCollectionMethod.lfs
me_egad:sampleCollectionMethod.lfs rdf:type owl:NamedIndividual ,
                                            me_egad:EGAD-SampleCollectionLocation ;
                                   rdfs:label "LOW-FLOW SAMPLE" .


###  http://sawgraph.spatialai.org/v1/me-egad#sampleCollectionMethod.lfsm
me_egad:sampleCollectionMethod.lfsm rdf:type owl:NamedIndividual ,
                                             me_egad:EGAD-SampleCollectionLocation ;
                                    rdfs:label "LOW-FLOW SAMPLE - MODIFIED" .


###  http://sawgraph.spatialai.org/v1/me-egad#sampleCollectionMethod.ls
me_egad:sampleCollectionMethod.ls rdf:type owl:NamedIndividual ,
                                           me_egad:EGAD-SampleCollectionLocation ;
                                  rdfs:label "LOW ACCURACY SURVEY" .


###  http://sawgraph.spatialai.org/v1/me-egad#sampleCollectionMethod.lsp
me_egad:sampleCollectionMethod.lsp rdf:type owl:NamedIndividual ,
                                            me_egad:EGAD-SampleCollectionLocation ;
                                   rdfs:label "LOG SCRAPINGS" .


###  http://sawgraph.spatialai.org/v1/me-egad#sampleCollectionMethod.lsp1
me_egad:sampleCollectionMethod.lsp1 rdf:type owl:NamedIndividual ,
                                             me_egad:EGAD-SampleCollectionLocation ;
                                    rdfs:label "LOG SCRAPINGS 1 INCH CIRCLES" .


###  http://sawgraph.spatialai.org/v1/me-egad#sampleCollectionMethod.lum
me_egad:sampleCollectionMethod.lum rdf:type owl:NamedIndividual ,
                                            me_egad:EGAD-SampleCollectionLocation ;
                                   rdfs:label "LUMEX - PORTABLE MERCURY VAPOR ANALYZER" .


###  http://sawgraph.spatialai.org/v1/me-egad#sampleCollectionMethod.m
me_egad:sampleCollectionMethod.m rdf:type owl:NamedIndividual ,
                                          me_egad:EGAD-SampleCollectionLocation ;
                                 rdfs:label "MEASURED" .


###  http://sawgraph.spatialai.org/v1/me-egad#sampleCollectionMethod.mh
me_egad:sampleCollectionMethod.mh rdf:type owl:NamedIndividual ,
                                           me_egad:EGAD-SampleCollectionLocation ;
                                  rdfs:label "MULTIHABITAT" .


###  http://sawgraph.spatialai.org/v1/me-egad#sampleCollectionMethod.mqm
me_egad:sampleCollectionMethod.mqm rdf:type owl:NamedIndividual ,
                                            me_egad:EGAD-SampleCollectionLocation ;
                                   rdfs:label "MAINE QUALITATIVE METHOD" .


###  http://sawgraph.spatialai.org/v1/me-egad#sampleCollectionMethod.mt
me_egad:sampleCollectionMethod.mt rdf:type owl:NamedIndividual ,
                                           me_egad:EGAD-SampleCollectionLocation ;
                                  rdfs:label "MINNOW TRAP" .


###  http://sawgraph.spatialai.org/v1/me-egad#sampleCollectionMethod.na
me_egad:sampleCollectionMethod.na rdf:type owl:NamedIndividual ,
                                           me_egad:EGAD-SampleCollectionLocation ;
                                  rdfs:label "NOT APPLICABLE" .


###  http://sawgraph.spatialai.org/v1/me-egad#sampleCollectionMethod.np
me_egad:sampleCollectionMethod.np rdf:type owl:NamedIndividual ,
                                           me_egad:EGAD-SampleCollectionLocation ;
                                  rdfs:label "NO-PURGE SAMPLE" .


###  http://sawgraph.spatialai.org/v1/me-egad#sampleCollectionMethod.ns
me_egad:sampleCollectionMethod.ns rdf:type owl:NamedIndividual ,
                                           me_egad:EGAD-SampleCollectionLocation ;
                                  rdfs:label "NO SAMPLE TAKEN" .


###  http://sawgraph.spatialai.org/v1/me-egad#sampleCollectionMethod.o
me_egad:sampleCollectionMethod.o rdf:type owl:NamedIndividual ,
                                          me_egad:EGAD-SampleCollectionLocation ;
                                 rdfs:label "OTHER" .


###  http://sawgraph.spatialai.org/v1/me-egad#sampleCollectionMethod.obs
me_egad:sampleCollectionMethod.obs rdf:type owl:NamedIndividual ,
                                            me_egad:EGAD-SampleCollectionLocation ;
                                   rdfs:label "OBSERVATION" .


###  http://sawgraph.spatialai.org/v1/me-egad#sampleCollectionMethod.pdc
me_egad:sampleCollectionMethod.pdc rdf:type owl:NamedIndividual ,
                                            me_egad:EGAD-SampleCollectionLocation ;
                                   rdfs:label "PETRI DISH CORES" .


###  http://sawgraph.spatialai.org/v1/me-egad#sampleCollectionMethod.ped
me_egad:sampleCollectionMethod.ped rdf:type owl:NamedIndividual ,
                                            me_egad:EGAD-SampleCollectionLocation ;
                                   rdfs:label "PROFUNDAL ECKMAN DREDGE" .


###  http://sawgraph.spatialai.org/v1/me-egad#sampleCollectionMethod.per
me_egad:sampleCollectionMethod.per rdf:type owl:NamedIndividual ,
                                            me_egad:EGAD-SampleCollectionLocation ;
                                   rdfs:label "PERISTALTIC PUMP" .


###  http://sawgraph.spatialai.org/v1/me-egad#sampleCollectionMethod.pid
me_egad:sampleCollectionMethod.pid rdf:type owl:NamedIndividual ,
                                            me_egad:EGAD-SampleCollectionLocation ;
                                   rdfs:label "PHOTOIONIZATION DETECTOR - HAND HELD" .


###  http://sawgraph.spatialai.org/v1/me-egad#sampleCollectionMethod.pp
me_egad:sampleCollectionMethod.pp rdf:type owl:NamedIndividual ,
                                           me_egad:EGAD-SampleCollectionLocation ;
                                  rdfs:label "PURGE PUMP" .


###  http://sawgraph.spatialai.org/v1/me-egad#sampleCollectionMethod.ppm
me_egad:sampleCollectionMethod.ppm rdf:type owl:NamedIndividual ,
                                            me_egad:EGAD-SampleCollectionLocation ;
                                   rdfs:label "PERIPHYTOMETER" .


###  http://sawgraph.spatialai.org/v1/me-egad#sampleCollectionMethod.pr
me_egad:sampleCollectionMethod.pr rdf:type owl:NamedIndividual ,
                                           me_egad:EGAD-SampleCollectionLocation ;
                                  rdfs:label "PLANT RUBBINGS" .


###  http://sawgraph.spatialai.org/v1/me-egad#sampleCollectionMethod.prd
me_egad:sampleCollectionMethod.prd rdf:type owl:NamedIndividual ,
                                            me_egad:EGAD-SampleCollectionLocation ;
                                   rdfs:label "PROFUNDAL ECKMAN DREDGE" .


###  http://sawgraph.spatialai.org/v1/me-egad#sampleCollectionMethod.ps
me_egad:sampleCollectionMethod.ps rdf:type owl:NamedIndividual ,
                                           me_egad:EGAD-SampleCollectionLocation ;
                                  rdfs:label "PACKER SAMPLE" .


###  http://sawgraph.spatialai.org/v1/me-egad#sampleCollectionMethod.pst
me_egad:sampleCollectionMethod.pst rdf:type owl:NamedIndividual ,
                                            me_egad:EGAD-SampleCollectionLocation ;
                                   rdfs:label "PLUMBING SYSTEM" .


###  http://sawgraph.spatialai.org/v1/me-egad#sampleCollectionMethod.pt
me_egad:sampleCollectionMethod.pt rdf:type owl:NamedIndividual ,
                                           me_egad:EGAD-SampleCollectionLocation ;
                                  rdfs:label "PUMP TIME" .


###  http://sawgraph.spatialai.org/v1/me-egad#sampleCollectionMethod.pws
me_egad:sampleCollectionMethod.pws rdf:type owl:NamedIndividual ,
                                            me_egad:EGAD-SampleCollectionLocation ;
                                   rdfs:label "PORE WATER SAMPLER" .


###  http://sawgraph.spatialai.org/v1/me-egad#sampleCollectionMethod.pwsp
me_egad:sampleCollectionMethod.pwsp rdf:type owl:NamedIndividual ,
                                             me_egad:EGAD-SampleCollectionLocation ;
                                    rdfs:label "PORE WATER SAMPLER WITH PURGE PUMP" .


###  http://sawgraph.spatialai.org/v1/me-egad#sampleCollectionMethod.rb
me_egad:sampleCollectionMethod.rb rdf:type owl:NamedIndividual ,
                                           me_egad:EGAD-SampleCollectionLocation ;
                                  rdfs:label "ROCK BASKET" .


###  http://sawgraph.spatialai.org/v1/me-egad#sampleCollectionMethod.rbg
me_egad:sampleCollectionMethod.rbg rdf:type owl:NamedIndividual ,
                                            me_egad:EGAD-SampleCollectionLocation ;
                                   rdfs:label "ROCK BAG" .


###  http://sawgraph.spatialai.org/v1/me-egad#sampleCollectionMethod.rcs
me_egad:sampleCollectionMethod.rcs rdf:type owl:NamedIndividual ,
                                            me_egad:EGAD-SampleCollectionLocation ;
                                   rdfs:label "ROCK/CWD SCRAPE" .


###  http://sawgraph.spatialai.org/v1/me-egad#sampleCollectionMethod.rsns
me_egad:sampleCollectionMethod.rsns rdf:type owl:NamedIndividual ,
                                             me_egad:EGAD-SampleCollectionLocation ;
                                    rdfs:label "ROCK/CWD SCRAPE AND D FRAME NET SWEEP" .


###  http://sawgraph.spatialai.org/v1/me-egad#sampleCollectionMethod.rsp
me_egad:sampleCollectionMethod.rsp rdf:type owl:NamedIndividual ,
                                            me_egad:EGAD-SampleCollectionLocation ;
                                   rdfs:label "ROCK SCRAPINGS" .


###  http://sawgraph.spatialai.org/v1/me-egad#sampleCollectionMethod.rsp1
me_egad:sampleCollectionMethod.rsp1 rdf:type owl:NamedIndividual ,
                                             me_egad:EGAD-SampleCollectionLocation ;
                                    rdfs:label "ROCK SCRAPINGS 1 INCH CIRCLES" .


###  http://sawgraph.spatialai.org/v1/me-egad#sampleCollectionMethod.rspf
me_egad:sampleCollectionMethod.rspf rdf:type owl:NamedIndividual ,
                                             me_egad:EGAD-SampleCollectionLocation ;
                                    rdfs:label "ROCK SCRAPINGS FOIL" .


###  http://sawgraph.spatialai.org/v1/me-egad#sampleCollectionMethod.s
me_egad:sampleCollectionMethod.s rdf:type owl:NamedIndividual ,
                                          me_egad:EGAD-SampleCollectionLocation ;
                                 rdfs:label "SLIDES" .


###  http://sawgraph.spatialai.org/v1/me-egad#sampleCollectionMethod.sb
me_egad:sampleCollectionMethod.sb rdf:type owl:NamedIndividual ,
                                           me_egad:EGAD-SampleCollectionLocation ;
                                  rdfs:label "SURBER" .


###  http://sawgraph.spatialai.org/v1/me-egad#sampleCollectionMethod.sd
me_egad:sampleCollectionMethod.sd rdf:type owl:NamedIndividual ,
                                           me_egad:EGAD-SampleCollectionLocation ;
                                  rdfs:label "SUCTION DEVICE" .


###  http://sawgraph.spatialai.org/v1/me-egad#sampleCollectionMethod.sd1
me_egad:sampleCollectionMethod.sd1 rdf:type owl:NamedIndividual ,
                                            me_egad:EGAD-SampleCollectionLocation ;
                                   rdfs:label "SECCHI DISK NO SCOPE" .


###  http://sawgraph.spatialai.org/v1/me-egad#sampleCollectionMethod.sd2
me_egad:sampleCollectionMethod.sd2 rdf:type owl:NamedIndividual ,
                                            me_egad:EGAD-SampleCollectionLocation ;
                                   rdfs:label "SECCHI DISK FLAT GLASS NO MASK" .


###  http://sawgraph.spatialai.org/v1/me-egad#sampleCollectionMethod.sd3
me_egad:sampleCollectionMethod.sd3 rdf:type owl:NamedIndividual ,
                                            me_egad:EGAD-SampleCollectionLocation ;
                                   rdfs:label "SECCHI DISK SLANT GLASS NO MASK" .


###  http://sawgraph.spatialai.org/v1/me-egad#sampleCollectionMethod.sd4
me_egad:sampleCollectionMethod.sd4 rdf:type owl:NamedIndividual ,
                                            me_egad:EGAD-SampleCollectionLocation ;
                                   rdfs:label "SECCHI DISK SLANT GLASS MASK" .


###  http://sawgraph.spatialai.org/v1/me-egad#sampleCollectionMethod.sd5
me_egad:sampleCollectionMethod.sd5 rdf:type owl:NamedIndividual ,
                                            me_egad:EGAD-SampleCollectionLocation ;
                                   rdfs:label "SECCHI DISK FLAT GLASS MASK" .


###  http://sawgraph.spatialai.org/v1/me-egad#sampleCollectionMethod.sd6
me_egad:sampleCollectionMethod.sd6 rdf:type owl:NamedIndividual ,
                                            me_egad:EGAD-SampleCollectionLocation ;
                                   rdfs:label "SECCHI DISK 8 IN DIA SLANT GLASS MASK" .


###  http://sawgraph.spatialai.org/v1/me-egad#sampleCollectionMethod.sd7
me_egad:sampleCollectionMethod.sd7 rdf:type owl:NamedIndividual ,
                                            me_egad:EGAD-SampleCollectionLocation ;
                                   rdfs:label "SECCHI DISK 20 CM" .


###  http://sawgraph.spatialai.org/v1/me-egad#sampleCollectionMethod.sg
me_egad:sampleCollectionMethod.sg rdf:type owl:NamedIndividual ,
                                           me_egad:EGAD-SampleCollectionLocation ;
                                  rdfs:label "STAFF GAUGE" .


###  http://sawgraph.spatialai.org/v1/me-egad#sampleCollectionMethod.sp
me_egad:sampleCollectionMethod.sp rdf:type owl:NamedIndividual ,
                                           me_egad:EGAD-SampleCollectionLocation ;
                                  rdfs:label "STOVEPIPE" .


###  http://sawgraph.spatialai.org/v1/me-egad#sampleCollectionMethod.ss
me_egad:sampleCollectionMethod.ss rdf:type owl:NamedIndividual ,
                                           me_egad:EGAD-SampleCollectionLocation ;
                                  rdfs:label "STORM SAMPLER" .


###  http://sawgraph.spatialai.org/v1/me-egad#sampleCollectionMethod.sum
me_egad:sampleCollectionMethod.sum rdf:type owl:NamedIndividual ,
                                            me_egad:EGAD-SampleCollectionLocation ;
                                   rdfs:label "SUMMA CANNISTER" .


###  http://sawgraph.spatialai.org/v1/me-egad#sampleCollectionMethod.t
me_egad:sampleCollectionMethod.t rdf:type owl:NamedIndividual ,
                                          me_egad:EGAD-SampleCollectionLocation ;
                                 rdfs:label "TRAP" .


###  http://sawgraph.spatialai.org/v1/me-egad#sampleCollectionMethod.ted
me_egad:sampleCollectionMethod.ted rdf:type owl:NamedIndividual ,
                                            me_egad:EGAD-SampleCollectionLocation ;
                                   rdfs:label "TEDLAR BAG" .


###  http://sawgraph.spatialai.org/v1/me-egad#sampleCollectionMethod.tn
me_egad:sampleCollectionMethod.tn rdf:type owl:NamedIndividual ,
                                           me_egad:EGAD-SampleCollectionLocation ;
                                  rdfs:label "TRAP NET" .


###  http://sawgraph.spatialai.org/v1/me-egad#sampleCollectionMethod.unk
me_egad:sampleCollectionMethod.unk rdf:type owl:NamedIndividual ,
                                            me_egad:EGAD-SampleCollectionLocation ;
                                   rdfs:label "UNKNOWN" .


###  http://sawgraph.spatialai.org/v1/me-egad#sampleCollectionMethod.vd
me_egad:sampleCollectionMethod.vd rdf:type owl:NamedIndividual ,
                                           me_egad:EGAD-SampleCollectionLocation ;
                                  rdfs:label "VAN DORN" .


###  http://sawgraph.spatialai.org/v1/me-egad#sampleCollectionMethod.vfr
me_egad:sampleCollectionMethod.vfr rdf:type owl:NamedIndividual ,
                                            me_egad:EGAD-SampleCollectionLocation ;
                                   rdfs:label "VARIABLE FLOW RATE PUMP" .


###  http://sawgraph.spatialai.org/v1/me-egad#sampleCollectionMethod.vw
me_egad:sampleCollectionMethod.vw rdf:type owl:NamedIndividual ,
                                           me_egad:EGAD-SampleCollectionLocation ;
                                  rdfs:label "VIBRATING WIRE" .


###  http://sawgraph.spatialai.org/v1/me-egad#sampleCollectionMethod.w
me_egad:sampleCollectionMethod.w rdf:type owl:NamedIndividual ,
                                          me_egad:EGAD-SampleCollectionLocation ;
                                 rdfs:label "WIPE SAMPLE" .


###  http://sawgraph.spatialai.org/v1/me-egad#sampleCollectionMethod.wl
me_egad:sampleCollectionMethod.wl rdf:type owl:NamedIndividual ,
                                           me_egad:EGAD-SampleCollectionLocation ;
                                  rdfs:label "WATER LEVEL METER" .


###  http://sawgraph.spatialai.org/v1/me-egad#sampleCollectionMethod.wqs
me_egad:sampleCollectionMethod.wqs rdf:type owl:NamedIndividual ,
                                            me_egad:EGAD-SampleCollectionLocation ;
                                   rdfs:label "DEP WATER QUALITY SAMPLER" .


###  http://sawgraph.spatialai.org/v1/me-egad#sampleLocation.af
me_egad:sampleLocation.af rdf:type owl:NamedIndividual ,
                                   me_egad:EGAD-SampleLocation ;
                          rdfs:label "AFTER FILTERS" .


###  http://sawgraph.spatialai.org/v1/me-egad#sampleLocation.as
me_egad:sampleLocation.as rdf:type owl:NamedIndividual ,
                                   me_egad:EGAD-SampleLocation ;
                          rdfs:label "AFTER SOFTENER" .


###  http://sawgraph.spatialai.org/v1/me-egad#sampleLocation.at
me_egad:sampleLocation.at rdf:type owl:NamedIndividual ,
                                   me_egad:EGAD-SampleLocation ;
                          rdfs:label "ATTIC" .


###  http://sawgraph.spatialai.org/v1/me-egad#sampleLocation.b
me_egad:sampleLocation.b rdf:type owl:NamedIndividual ,
                                  me_egad:EGAD-SampleLocation ;
                         rdfs:label "BANK" .


###  http://sawgraph.spatialai.org/v1/me-egad#sampleLocation.bao
me_egad:sampleLocation.bao rdf:type owl:NamedIndividual ,
                                    me_egad:EGAD-SampleLocation ;
                           rdfs:label "BATH IN OTHER" .


###  http://sawgraph.spatialai.org/v1/me-egad#sampleLocation.bd
me_egad:sampleLocation.bd rdf:type owl:NamedIndividual ,
                                   me_egad:EGAD-SampleLocation ;
                          rdfs:label "BENEATH DISPENSER" .


###  http://sawgraph.spatialai.org/v1/me-egad#sampleLocation.be
me_egad:sampleLocation.be rdf:type owl:NamedIndividual ,
                                   me_egad:EGAD-SampleLocation ;
                          rdfs:label "BEFORE FILTERS" .


###  http://sawgraph.spatialai.org/v1/me-egad#sampleLocation.biwb
me_egad:sampleLocation.biwb rdf:type owl:NamedIndividual ,
                                     me_egad:EGAD-SampleLocation ;
                            rdfs:label "BATH IN WELL BOAT" .


###  http://sawgraph.spatialai.org/v1/me-egad#sampleLocation.bm
me_egad:sampleLocation.bm rdf:type owl:NamedIndividual ,
                                   me_egad:EGAD-SampleLocation ;
                          rdfs:label "BASEMENT" .


###  http://sawgraph.spatialai.org/v1/me-egad#sampleLocation.bp
me_egad:sampleLocation.bp rdf:type owl:NamedIndividual ,
                                   me_egad:EGAD-SampleLocation ;
                          rdfs:label "BENEATH PIPING" .


###  http://sawgraph.spatialai.org/v1/me-egad#sampleLocation.br
me_egad:sampleLocation.br rdf:type owl:NamedIndividual ,
                                   me_egad:EGAD-SampleLocation ;
                          rdfs:label "BRIDGE" .


###  http://sawgraph.spatialai.org/v1/me-egad#sampleLocation.bt
me_egad:sampleLocation.bt rdf:type owl:NamedIndividual ,
                                   me_egad:EGAD-SampleLocation ;
                          rdfs:label "BETWEEN FILTERS" .


###  http://sawgraph.spatialai.org/v1/me-egad#sampleLocation.c
me_egad:sampleLocation.c rdf:type owl:NamedIndividual ,
                                  me_egad:EGAD-SampleLocation ;
                         rdfs:label "CULVERT" .


###  http://sawgraph.spatialai.org/v1/me-egad#sampleLocation.cw
me_egad:sampleLocation.cw rdf:type owl:NamedIndividual ,
                                   me_egad:EGAD-SampleLocation ;
                          rdfs:label "CRAWLSPACE" .


###  http://sawgraph.spatialai.org/v1/me-egad#sampleLocation.d
me_egad:sampleLocation.d rdf:type owl:NamedIndividual ,
                                  me_egad:EGAD-SampleLocation ;
                         rdfs:label "DOCK" .


###  http://sawgraph.spatialai.org/v1/me-egad#sampleLocation.ebag
me_egad:sampleLocation.ebag rdf:type owl:NamedIndividual ,
                                     me_egad:EGAD-SampleLocation ;
                            rdfs:label "ENGINEERED MEMBRANE BAG" .


###  http://sawgraph.spatialai.org/v1/me-egad#sampleLocation.ef
me_egad:sampleLocation.ef rdf:type owl:NamedIndividual ,
                                   me_egad:EGAD-SampleLocation ;
                          rdfs:label "TREATMENT SYSTEM - EFFLUENT" .


###  http://sawgraph.spatialai.org/v1/me-egad#sampleLocation.f
me_egad:sampleLocation.f rdf:type owl:NamedIndividual ,
                                  me_egad:EGAD-SampleLocation ;
                         rdfs:label "FLOOR" .


###  http://sawgraph.spatialai.org/v1/me-egad#sampleLocation.fe
me_egad:sampleLocation.fe rdf:type owl:NamedIndividual ,
                                   me_egad:EGAD-SampleLocation ;
                          rdfs:label "FEED" .


###  http://sawgraph.spatialai.org/v1/me-egad#sampleLocation.ff
me_egad:sampleLocation.ff rdf:type owl:NamedIndividual ,
                                   me_egad:EGAD-SampleLocation ;
                          rdfs:label "FIRST FLOOR" .


###  http://sawgraph.spatialai.org/v1/me-egad#sampleLocation.gr
me_egad:sampleLocation.gr rdf:type owl:NamedIndividual ,
                                   me_egad:EGAD-SampleLocation ;
                          rdfs:label "GARAGE" .


###  http://sawgraph.spatialai.org/v1/me-egad#sampleLocation.in
me_egad:sampleLocation.in rdf:type owl:NamedIndividual ,
                                   me_egad:EGAD-SampleLocation ;
                          rdfs:label "TREATMENT SYSTEM - INFLUENT" .


###  http://sawgraph.spatialai.org/v1/me-egad#sampleLocation.mh
me_egad:sampleLocation.mh rdf:type owl:NamedIndividual ,
                                   me_egad:EGAD-SampleLocation ;
                          rdfs:label "MANHOLE" .


###  http://sawgraph.spatialai.org/v1/me-egad#sampleLocation.mp
me_egad:sampleLocation.mp rdf:type owl:NamedIndividual ,
                                   me_egad:EGAD-SampleLocation ;
                          rdfs:label "TREATMENT SYSTEM - MIDPOINT" .


###  http://sawgraph.spatialai.org/v1/me-egad#sampleLocation.na
me_egad:sampleLocation.na rdf:type owl:NamedIndividual ,
                                   me_egad:EGAD-SampleLocation ;
                          rdfs:label "NOT APPLICABLE" .


###  http://sawgraph.spatialai.org/v1/me-egad#sampleLocation.o
me_egad:sampleLocation.o rdf:type owl:NamedIndividual ,
                                  me_egad:EGAD-SampleLocation ;
                         rdfs:label "OTHER" .


###  http://sawgraph.spatialai.org/v1/me-egad#sampleLocation.od
me_egad:sampleLocation.od rdf:type owl:NamedIndividual ,
                                   me_egad:EGAD-SampleLocation ;
                          rdfs:label "OUTDOOR AIR" .


###  http://sawgraph.spatialai.org/v1/me-egad#sampleLocation.ot
me_egad:sampleLocation.ot rdf:type owl:NamedIndividual ,
                                   me_egad:EGAD-SampleLocation ;
                          rdfs:label "OUTSIDE TAP" .


###  http://sawgraph.spatialai.org/v1/me-egad#sampleLocation.pm
me_egad:sampleLocation.pm rdf:type owl:NamedIndividual ,
                                   me_egad:EGAD-SampleLocation ;
                          rdfs:label "POST TREATMENT METALS (SAMPLED AFTER TREATMENT SYSTEM FOR IRON, MANGANESE ETC)" .


###  http://sawgraph.spatialai.org/v1/me-egad#sampleLocation.pt
me_egad:sampleLocation.pt rdf:type owl:NamedIndividual ,
                                   me_egad:EGAD-SampleLocation ;
                          rdfs:label "PRESSURE TANK" .


###  http://sawgraph.spatialai.org/v1/me-egad#sampleLocation.pu
me_egad:sampleLocation.pu rdf:type owl:NamedIndividual ,
                                   me_egad:EGAD-SampleLocation ;
                          rdfs:label "WELLHEAD" .


###  http://sawgraph.spatialai.org/v1/me-egad#sampleLocation.sa
me_egad:sampleLocation.sa rdf:type owl:NamedIndividual ,
                                   me_egad:EGAD-SampleLocation ;
                          rdfs:label "SIDE WALL ABOVE 2 FEET" .


###  http://sawgraph.spatialai.org/v1/me-egad#sampleLocation.sb
me_egad:sampleLocation.sb rdf:type owl:NamedIndividual ,
                                   me_egad:EGAD-SampleLocation ;
                          rdfs:label "SIDE WALL BELOW 2 FEET" .


###  http://sawgraph.spatialai.org/v1/me-egad#sampleLocation.sf
me_egad:sampleLocation.sf rdf:type owl:NamedIndividual ,
                                   me_egad:EGAD-SampleLocation ;
                          rdfs:label "SECOND FLOOR" .


###  http://sawgraph.spatialai.org/v1/me-egad#sampleLocation.sh
me_egad:sampleLocation.sh rdf:type owl:NamedIndividual ,
                                   me_egad:EGAD-SampleLocation ;
                          rdfs:label "SHORE ACCESS" .


###  http://sawgraph.spatialai.org/v1/me-egad#sampleLocation.ss
me_egad:sampleLocation.ss rdf:type owl:NamedIndividual ,
                                   me_egad:EGAD-SampleLocation ;
                          rdfs:label "SUBSLAB" .


###  http://sawgraph.spatialai.org/v1/me-egad#sampleLocation.st
me_egad:sampleLocation.st rdf:type owl:NamedIndividual ,
                                   me_egad:EGAD-SampleLocation ;
                          rdfs:label "SUBTIDAL" .


###  http://sawgraph.spatialai.org/v1/me-egad#sampleLocation.sw
me_egad:sampleLocation.sw rdf:type owl:NamedIndividual ,
                                   me_egad:EGAD-SampleLocation ;
                          rdfs:label "STAIRWAY" .


###  http://sawgraph.spatialai.org/v1/me-egad#sampleLocation.t
me_egad:sampleLocation.t rdf:type owl:NamedIndividual ,
                                  me_egad:EGAD-SampleLocation ;
                         rdfs:label "INSIDE TAP" .


###  http://sawgraph.spatialai.org/v1/me-egad#sampleLocation.tf
me_egad:sampleLocation.tf rdf:type owl:NamedIndividual ,
                                   me_egad:EGAD-SampleLocation ;
                          rdfs:label "THIRD FLOOR" .


###  http://sawgraph.spatialai.org/v1/me-egad#sampleLocation.u
me_egad:sampleLocation.u rdf:type owl:NamedIndividual ,
                                  me_egad:EGAD-SampleLocation ;
                         rdfs:label "UNKNOWN" .


###  http://sawgraph.spatialai.org/v1/me-egad#sampleLocation.w
me_egad:sampleLocation.w rdf:type owl:NamedIndividual ,
                                  me_egad:EGAD-SampleLocation ;
                         rdfs:label "WADING" .


###  http://sawgraph.spatialai.org/v1/me-egad#samplePointType.acs
me_egad:samplePointType.acs rdf:type owl:NamedIndividual ,
                                     me_egad:EGAD-SamplePointType ;
                            rdfs:label "ASPHALT/CONCRETE SURFACE" .


###  http://sawgraph.spatialai.org/v1/me-egad#samplePointType.aquaf
me_egad:samplePointType.aquaf rdf:type owl:NamedIndividual ,
                                       me_egad:EGAD-SamplePointType ;
                              rdfs:label "AQUACULTURE FACILITY" .


###  http://sawgraph.spatialai.org/v1/me-egad#samplePointType.aquap
me_egad:samplePointType.aquap rdf:type owl:NamedIndividual ,
                                       me_egad:EGAD-SamplePointType ;
                              rdfs:label "AQUACULTURE PEN" .


###  http://sawgraph.spatialai.org/v1/me-egad#samplePointType.ast
me_egad:samplePointType.ast rdf:type owl:NamedIndividual ,
                                     me_egad:EGAD-SamplePointType ;
                            rdfs:label "ABOVEGROUND STORAGE TANK" .


###  http://sawgraph.spatialai.org/v1/me-egad#samplePointType.aw
me_egad:samplePointType.aw rdf:type owl:NamedIndividual ,
                                    me_egad:EGAD-SamplePointType ;
                           rdfs:label "AGRICULTURAL WELL" .


###  http://sawgraph.spatialai.org/v1/me-egad#samplePointType.bc
me_egad:samplePointType.bc rdf:type owl:NamedIndividual ,
                                    me_egad:EGAD-SamplePointType ;
                           rdfs:label "BEACH" .


###  http://sawgraph.spatialai.org/v1/me-egad#samplePointType.bldg
me_egad:samplePointType.bldg rdf:type owl:NamedIndividual ,
                                      me_egad:EGAD-SamplePointType ;
                             rdfs:label "BUILDING" .


###  http://sawgraph.spatialai.org/v1/me-egad#samplePointType.bow
me_egad:samplePointType.bow rdf:type owl:NamedIndividual ,
                                     me_egad:EGAD-SamplePointType ;
                            rdfs:label "BACKFILL OBSERVATION WELL" .


###  http://sawgraph.spatialai.org/v1/me-egad#samplePointType.br
me_egad:samplePointType.br rdf:type owl:NamedIndividual ,
                                    me_egad:EGAD-SamplePointType ;
                           rdfs:label "BARN" .


###  http://sawgraph.spatialai.org/v1/me-egad#samplePointType.bs
me_egad:samplePointType.bs rdf:type owl:NamedIndividual ,
                                    me_egad:EGAD-SamplePointType ;
                           rdfs:label "BUILDING SUMP" .


###  http://sawgraph.spatialai.org/v1/me-egad#samplePointType.bt
me_egad:samplePointType.bt rdf:type owl:NamedIndividual ,
                                    me_egad:EGAD-SamplePointType ;
                           rdfs:label "BULK MILK TANK" .


###  http://sawgraph.spatialai.org/v1/me-egad#samplePointType.cb
me_egad:samplePointType.cb rdf:type owl:NamedIndividual ,
                                    me_egad:EGAD-SamplePointType ;
                           rdfs:label "CATCH BASIN" .


###  http://sawgraph.spatialai.org/v1/me-egad#samplePointType.ct
me_egad:samplePointType.ct rdf:type owl:NamedIndividual ,
                                    me_egad:EGAD-SamplePointType ;
                           rdfs:label "COLLECTION TRENCH" .


###  http://sawgraph.spatialai.org/v1/me-egad#samplePointType.dm
me_egad:samplePointType.dm rdf:type owl:NamedIndividual ,
                                    me_egad:EGAD-SamplePointType ;
                           rdfs:label "DRUM" .


###  http://sawgraph.spatialai.org/v1/me-egad#samplePointType.dp
me_egad:samplePointType.dp rdf:type owl:NamedIndividual ,
                                    me_egad:EGAD-SamplePointType ;
                           rdfs:label "DETENTION POND" .


###  http://sawgraph.spatialai.org/v1/me-egad#samplePointType.dt
me_egad:samplePointType.dt rdf:type owl:NamedIndividual ,
                                    me_egad:EGAD-SamplePointType ;
                           rdfs:label "DITCH" .


###  http://sawgraph.spatialai.org/v1/me-egad#samplePointType.dws
me_egad:samplePointType.dws rdf:type owl:NamedIndividual ,
                                     me_egad:EGAD-SamplePointType ;
                            rdfs:label "DISCONTINUED WATER SUPPLY (I.E. WELL EXISTS BUT NOT USED FOR DRINKING WATER)" .


###  http://sawgraph.spatialai.org/v1/me-egad#samplePointType.esw
me_egad:samplePointType.esw rdf:type owl:NamedIndividual ,
                                     me_egad:EGAD-SamplePointType ;
                            rdfs:label "ESTUARY" .


###  http://sawgraph.spatialai.org/v1/me-egad#samplePointType.ew
me_egad:samplePointType.ew rdf:type owl:NamedIndividual ,
                                    me_egad:EGAD-SamplePointType ;
                           rdfs:label "EXTRACTION WELL" .


###  http://sawgraph.spatialai.org/v1/me-egad#samplePointType.ewm
me_egad:samplePointType.ewm rdf:type owl:NamedIndividual ,
                                     me_egad:EGAD-SamplePointType ;
                            rdfs:label "EXTRACTION WELL MANIFOLD" .


###  http://sawgraph.spatialai.org/v1/me-egad#samplePointType.exs
me_egad:samplePointType.exs rdf:type owl:NamedIndividual ,
                                     me_egad:EGAD-SamplePointType ;
                            rdfs:label "EXCAVATION SOIL" .


###  http://sawgraph.spatialai.org/v1/me-egad#samplePointType.exw
me_egad:samplePointType.exw rdf:type owl:NamedIndividual ,
                                     me_egad:EGAD-SamplePointType ;
                            rdfs:label "EXCAVATION GROUNDWATER" .


###  http://sawgraph.spatialai.org/v1/me-egad#samplePointType.fb
me_egad:samplePointType.fb rdf:type owl:NamedIndividual ,
                                    me_egad:EGAD-SamplePointType ;
                           rdfs:label "FEED BUNK" .


###  http://sawgraph.spatialai.org/v1/me-egad#samplePointType.ff
me_egad:samplePointType.ff rdf:type owl:NamedIndividual ,
                                    me_egad:EGAD-SamplePointType ;
                           rdfs:label "FARM FIELD" .


###  http://sawgraph.spatialai.org/v1/me-egad#samplePointType.fht
me_egad:samplePointType.fht rdf:type owl:NamedIndividual ,
                                     me_egad:EGAD-SamplePointType ;
                            rdfs:label "FISH HATCHERY TANK" .


###  http://sawgraph.spatialai.org/v1/me-egad#samplePointType.fl
me_egad:samplePointType.fl rdf:type owl:NamedIndividual ,
                                    me_egad:EGAD-SamplePointType ;
                           rdfs:label "FLOWAGE" .


###  http://sawgraph.spatialai.org/v1/me-egad#samplePointType.flare
me_egad:samplePointType.flare rdf:type owl:NamedIndividual ,
                                       me_egad:EGAD-SamplePointType ;
                              rdfs:label "FLARE" .


###  http://sawgraph.spatialai.org/v1/me-egad#samplePointType.fldr
me_egad:samplePointType.fldr rdf:type owl:NamedIndividual ,
                                      me_egad:EGAD-SamplePointType ;
                             rdfs:label "FLOOR DRAIN" .


###  http://sawgraph.spatialai.org/v1/me-egad#samplePointType.fs
me_egad:samplePointType.fs rdf:type owl:NamedIndividual ,
                                    me_egad:EGAD-SamplePointType ;
                           rdfs:label "FARM STORAGE" .


###  http://sawgraph.spatialai.org/v1/me-egad#samplePointType.gect
me_egad:samplePointType.gect rdf:type owl:NamedIndividual ,
                                      me_egad:EGAD-SamplePointType ;
                             rdfs:label "GAS EXTRACTION CONDENSATE TRAP" .


###  http://sawgraph.spatialai.org/v1/me-egad#samplePointType.genp
me_egad:samplePointType.genp rdf:type owl:NamedIndividual ,
                                      me_egad:EGAD-SamplePointType ;
                             rdfs:label "GAS ENERGY PLANT" .


###  http://sawgraph.spatialai.org/v1/me-egad#samplePointType.geph
me_egad:samplePointType.geph rdf:type owl:NamedIndividual ,
                                      me_egad:EGAD-SamplePointType ;
                             rdfs:label "GAS EXTRACTION POINT HORIZONTAL" .


###  http://sawgraph.spatialai.org/v1/me-egad#samplePointType.gepl
me_egad:samplePointType.gepl rdf:type owl:NamedIndividual ,
                                      me_egad:EGAD-SamplePointType ;
                             rdfs:label "GAS EXTRACTION POINT LEACHATE" .


###  http://sawgraph.spatialai.org/v1/me-egad#samplePointType.gepv
me_egad:samplePointType.gepv rdf:type owl:NamedIndividual ,
                                      me_egad:EGAD-SamplePointType ;
                             rdfs:label "GAS EXTRACTION POINT VERTICAL" .


###  http://sawgraph.spatialai.org/v1/me-egad#samplePointType.gesgv
me_egad:samplePointType.gesgv rdf:type owl:NamedIndividual ,
                                       me_egad:EGAD-SamplePointType ;
                              rdfs:label "GAS EXTRACTION SUB-LINER GAS VENT" .


###  http://sawgraph.spatialai.org/v1/me-egad#samplePointType.gh
me_egad:samplePointType.gh rdf:type owl:NamedIndividual ,
                                    me_egad:EGAD-SamplePointType ;
                           rdfs:label "GREENHOUSE" .


###  http://sawgraph.spatialai.org/v1/me-egad#samplePointType.gm
me_egad:samplePointType.gm rdf:type owl:NamedIndividual ,
                                    me_egad:EGAD-SamplePointType ;
                           rdfs:label "GAS MONITOR" .


###  http://sawgraph.spatialai.org/v1/me-egad#samplePointType.gp
me_egad:samplePointType.gp rdf:type owl:NamedIndividual ,
                                    me_egad:EGAD-SamplePointType ;
                           rdfs:label "GEOPROBE" .


###  http://sawgraph.spatialai.org/v1/me-egad#samplePointType.gr
me_egad:samplePointType.gr rdf:type owl:NamedIndividual ,
                                    me_egad:EGAD-SamplePointType ;
                           rdfs:label "GARDEN" .


###  http://sawgraph.spatialai.org/v1/me-egad#samplePointType.h2s
me_egad:samplePointType.h2s rdf:type owl:NamedIndividual ,
                                     me_egad:EGAD-SamplePointType ;
                            rdfs:label "H2S MONITOR" .


###  http://sawgraph.spatialai.org/v1/me-egad#samplePointType.ht
me_egad:samplePointType.ht rdf:type owl:NamedIndividual ,
                                    me_egad:EGAD-SamplePointType ;
                           rdfs:label "HIGH TUNNEL" .


###  http://sawgraph.spatialai.org/v1/me-egad#samplePointType.hv
me_egad:samplePointType.hv rdf:type owl:NamedIndividual ,
                                    me_egad:EGAD-SamplePointType ;
                           rdfs:label "HIVES" .


###  http://sawgraph.spatialai.org/v1/me-egad#samplePointType.im
me_egad:samplePointType.im rdf:type owl:NamedIndividual ,
                                    me_egad:EGAD-SamplePointType ;
                           rdfs:label "IMPOUNDMENT" .


###  http://sawgraph.spatialai.org/v1/me-egad#samplePointType.iw
me_egad:samplePointType.iw rdf:type owl:NamedIndividual ,
                                    me_egad:EGAD-SamplePointType ;
                           rdfs:label "INJECTION WELL" .


###  http://sawgraph.spatialai.org/v1/me-egad#samplePointType.iwsw
me_egad:samplePointType.iwsw rdf:type owl:NamedIndividual ,
                                      me_egad:EGAD-SamplePointType ;
                             rdfs:label "INDUSTRIAL WATER SUPPLY WELL" .


###  http://sawgraph.spatialai.org/v1/me-egad#samplePointType.lds
me_egad:samplePointType.lds rdf:type owl:NamedIndividual ,
                                     me_egad:EGAD-SamplePointType ;
                            rdfs:label "LEAK DETECTION SYSTEM" .


###  http://sawgraph.spatialai.org/v1/me-egad#samplePointType.lfssep
me_egad:samplePointType.lfssep rdf:type owl:NamedIndividual ,
                                        me_egad:EGAD-SamplePointType ;
                               rdfs:label "LANDFILL SURFACE SCAN EMISSION POINT" .


###  http://sawgraph.spatialai.org/v1/me-egad#samplePointType.lg
me_egad:samplePointType.lg rdf:type owl:NamedIndividual ,
                                    me_egad:EGAD-SamplePointType ;
                           rdfs:label "LAGOON" .


###  http://sawgraph.spatialai.org/v1/me-egad#samplePointType.lk
me_egad:samplePointType.lk rdf:type owl:NamedIndividual ,
                                    me_egad:EGAD-SamplePointType ;
                           rdfs:label "LAKE" .


###  http://sawgraph.spatialai.org/v1/me-egad#samplePointType.lpd
me_egad:samplePointType.lpd rdf:type owl:NamedIndividual ,
                                     me_egad:EGAD-SamplePointType ;
                            rdfs:label "LEACHATE POND" .


###  http://sawgraph.spatialai.org/v1/me-egad#samplePointType.lps
me_egad:samplePointType.lps rdf:type owl:NamedIndividual ,
                                     me_egad:EGAD-SamplePointType ;
                            rdfs:label "LEACHATE PUMP STATION" .


###  http://sawgraph.spatialai.org/v1/me-egad#samplePointType.ls
me_egad:samplePointType.ls rdf:type owl:NamedIndividual ,
                                    me_egad:EGAD-SamplePointType ;
                           rdfs:label "LEACHATE SYSTEM" .


###  http://sawgraph.spatialai.org/v1/me-egad#samplePointType.lsl
me_egad:samplePointType.lsl rdf:type owl:NamedIndividual ,
                                     me_egad:EGAD-SamplePointType ;
                            rdfs:label "LANDSPREAD SOIL" .


###  http://sawgraph.spatialai.org/v1/me-egad#samplePointType.lv
me_egad:samplePointType.lv rdf:type owl:NamedIndividual ,
                                    me_egad:EGAD-SamplePointType ;
                           rdfs:label "LANDFILL VENT" .


###  http://sawgraph.spatialai.org/v1/me-egad#samplePointType.met
me_egad:samplePointType.met rdf:type owl:NamedIndividual ,
                                     me_egad:EGAD-SamplePointType ;
                            rdfs:label "METEORLOGICAL STATION" .


###  http://sawgraph.spatialai.org/v1/me-egad#samplePointType.mh
me_egad:samplePointType.mh rdf:type owl:NamedIndividual ,
                                    me_egad:EGAD-SamplePointType ;
                           rdfs:label "MAN HOLE" .


###  http://sawgraph.spatialai.org/v1/me-egad#samplePointType.mi
me_egad:samplePointType.mi rdf:type owl:NamedIndividual ,
                                    me_egad:EGAD-SamplePointType ;
                           rdfs:label "MICRO-WELL" .


###  http://sawgraph.spatialai.org/v1/me-egad#samplePointType.misa
me_egad:samplePointType.misa rdf:type owl:NamedIndividual ,
                                      me_egad:EGAD-SamplePointType ;
                             rdfs:label "MULTI-INCREMENT SAMPLE AREA" .


###  http://sawgraph.spatialai.org/v1/me-egad#samplePointType.mp
me_egad:samplePointType.mp rdf:type owl:NamedIndividual ,
                                    me_egad:EGAD-SamplePointType ;
                           rdfs:label "MANURE PIT" .


###  http://sawgraph.spatialai.org/v1/me-egad#samplePointType.mrn
me_egad:samplePointType.mrn rdf:type owl:NamedIndividual ,
                                     me_egad:EGAD-SamplePointType ;
                            rdfs:label "MARINE" .


###  http://sawgraph.spatialai.org/v1/me-egad#samplePointType.muw
me_egad:samplePointType.muw rdf:type owl:NamedIndividual ,
                                     me_egad:EGAD-SamplePointType ;
                            rdfs:label "MULTI USE WELL" .


###  http://sawgraph.spatialai.org/v1/me-egad#samplePointType.mw
me_egad:samplePointType.mw rdf:type owl:NamedIndividual ,
                                    me_egad:EGAD-SamplePointType ;
                           rdfs:label "MONITORING WELL" .


###  http://sawgraph.spatialai.org/v1/me-egad#samplePointType.mx
me_egad:samplePointType.mx rdf:type owl:NamedIndividual ,
                                    me_egad:EGAD-SamplePointType ;
                           rdfs:label "MIXER WAGON" .


###  http://sawgraph.spatialai.org/v1/me-egad#samplePointType.or
me_egad:samplePointType.or rdf:type owl:NamedIndividual ,
                                    me_egad:EGAD-SamplePointType ;
                           rdfs:label "ORCHARD" .


###  http://sawgraph.spatialai.org/v1/me-egad#samplePointType.pd
me_egad:samplePointType.pd rdf:type owl:NamedIndividual ,
                                    me_egad:EGAD-SamplePointType ;
                           rdfs:label "POND" .


###  http://sawgraph.spatialai.org/v1/me-egad#samplePointType.pdk
me_egad:samplePointType.pdk rdf:type owl:NamedIndividual ,
                                     me_egad:EGAD-SamplePointType ;
                            rdfs:label "PADDOCK" .


###  http://sawgraph.spatialai.org/v1/me-egad#samplePointType.pi
me_egad:samplePointType.pi rdf:type owl:NamedIndividual ,
                                    me_egad:EGAD-SamplePointType ;
                           rdfs:label "PIEZOMETER" .


###  http://sawgraph.spatialai.org/v1/me-egad#samplePointType.pm
me_egad:samplePointType.pm rdf:type owl:NamedIndividual ,
                                    me_egad:EGAD-SamplePointType ;
                           rdfs:label "PROCESS MATERIAL" .


###  http://sawgraph.spatialai.org/v1/me-egad#samplePointType.pore
me_egad:samplePointType.pore rdf:type owl:NamedIndividual ,
                                      me_egad:EGAD-SamplePointType ;
                             rdfs:label "PORE WATER SAMPLER" .


###  http://sawgraph.spatialai.org/v1/me-egad#samplePointType.pows
me_egad:samplePointType.pows rdf:type owl:NamedIndividual ,
                                      me_egad:EGAD-SamplePointType ;
                             rdfs:label "PROCESS WATER" .


###  http://sawgraph.spatialai.org/v1/me-egad#samplePointType.pp
me_egad:samplePointType.pp rdf:type owl:NamedIndividual ,
                                    me_egad:EGAD-SamplePointType ;
                           rdfs:label "PUSH POINT" .


###  http://sawgraph.spatialai.org/v1/me-egad#samplePointType.prd
me_egad:samplePointType.prd rdf:type owl:NamedIndividual ,
                                     me_egad:EGAD-SamplePointType ;
                            rdfs:label "PERIMETER DRAIN" .


###  http://sawgraph.spatialai.org/v1/me-egad#samplePointType.prws
me_egad:samplePointType.prws rdf:type owl:NamedIndividual ,
                                      me_egad:EGAD-SamplePointType ;
                             rdfs:label "PRIVATE WATER SUPPLY - HISTORIC" .


###  http://sawgraph.spatialai.org/v1/me-egad#samplePointType.puwss
me_egad:samplePointType.puwss rdf:type owl:NamedIndividual ,
                                       me_egad:EGAD-SamplePointType ;
                              rdfs:label "PUBLIC WATER SUPPLY SURFACE" .


###  http://sawgraph.spatialai.org/v1/me-egad#samplePointType.puwsw
me_egad:samplePointType.puwsw rdf:type owl:NamedIndividual ,
                                       me_egad:EGAD-SamplePointType ;
                              rdfs:label "PUBLIC WATER SUPPLY WELL" .


###  http://sawgraph.spatialai.org/v1/me-egad#samplePointType.pws
me_egad:samplePointType.pws rdf:type owl:NamedIndividual ,
                                     me_egad:EGAD-SamplePointType ;
                            rdfs:label "PUBLIC WATER SUPPLY - HISTORIC" .


###  http://sawgraph.spatialai.org/v1/me-egad#samplePointType.pwss
me_egad:samplePointType.pwss rdf:type owl:NamedIndividual ,
                                      me_egad:EGAD-SamplePointType ;
                             rdfs:label "PRIVATE WATER SUPPLY SURFACE" .


###  http://sawgraph.spatialai.org/v1/me-egad#samplePointType.pwsw
me_egad:samplePointType.pwsw rdf:type owl:NamedIndividual ,
                                      me_egad:EGAD-SamplePointType ;
                             rdfs:label "PRIVATE WATER SUPPLY WELL" .


###  http://sawgraph.spatialai.org/v1/me-egad#samplePointType.qa
me_egad:samplePointType.qa rdf:type owl:NamedIndividual ,
                                    me_egad:EGAD-SamplePointType ;
                           rdfs:label "QA/QC" .


###  http://sawgraph.spatialai.org/v1/me-egad#samplePointType.qr
me_egad:samplePointType.qr rdf:type owl:NamedIndividual ,
                                    me_egad:EGAD-SamplePointType ;
                           rdfs:label "QUARRY" .


###  http://sawgraph.spatialai.org/v1/me-egad#samplePointType.re
me_egad:samplePointType.re rdf:type owl:NamedIndividual ,
                                    me_egad:EGAD-SamplePointType ;
                           rdfs:label "RESERVOIR" .


###  http://sawgraph.spatialai.org/v1/me-egad#samplePointType.ri
me_egad:samplePointType.ri rdf:type owl:NamedIndividual ,
                                    me_egad:EGAD-SamplePointType ;
                           rdfs:label "RIVER" .


###  http://sawgraph.spatialai.org/v1/me-egad#samplePointType.sa
me_egad:samplePointType.sa rdf:type owl:NamedIndividual ,
                                    me_egad:EGAD-SamplePointType ;
                           rdfs:label "SOIL AUGER" .


###  http://sawgraph.spatialai.org/v1/me-egad#samplePointType.sd
me_egad:samplePointType.sd rdf:type owl:NamedIndividual ,
                                    me_egad:EGAD-SamplePointType ;
                           rdfs:label "STORM DRAIN" .


###  http://sawgraph.spatialai.org/v1/me-egad#samplePointType.sgp
me_egad:samplePointType.sgp rdf:type owl:NamedIndividual ,
                                     me_egad:EGAD-SamplePointType ;
                            rdfs:label "SOIL GAS PROBE" .


###  http://sawgraph.spatialai.org/v1/me-egad#samplePointType.sl
me_egad:samplePointType.sl rdf:type owl:NamedIndividual ,
                                    me_egad:EGAD-SamplePointType ;
                           rdfs:label "SILO" .


###  http://sawgraph.spatialai.org/v1/me-egad#samplePointType.sm
me_egad:samplePointType.sm rdf:type owl:NamedIndividual ,
                                    me_egad:EGAD-SamplePointType ;
                           rdfs:label "SEEP MARSH" .


###  http://sawgraph.spatialai.org/v1/me-egad#samplePointType.sp
me_egad:samplePointType.sp rdf:type owl:NamedIndividual ,
                                    me_egad:EGAD-SamplePointType ;
                           rdfs:label "SEDIMENTATION POND" .


###  http://sawgraph.spatialai.org/v1/me-egad#samplePointType.spb
me_egad:samplePointType.spb rdf:type owl:NamedIndividual ,
                                     me_egad:EGAD-SamplePointType ;
                            rdfs:label "SPHAGNUM BOG" .


###  http://sawgraph.spatialai.org/v1/me-egad#samplePointType.spm
me_egad:samplePointType.spm rdf:type owl:NamedIndividual ,
                                     me_egad:EGAD-SamplePointType ;
                            rdfs:label "STOCKPILE MATERIAL" .


###  http://sawgraph.spatialai.org/v1/me-egad#samplePointType.spr
me_egad:samplePointType.spr rdf:type owl:NamedIndividual ,
                                     me_egad:EGAD-SamplePointType ;
                            rdfs:label "SPRING/SEEP" .


###  http://sawgraph.spatialai.org/v1/me-egad#samplePointType.spt
me_egad:samplePointType.spt rdf:type owl:NamedIndividual ,
                                     me_egad:EGAD-SamplePointType ;
                            rdfs:label "SEPTIC TANK" .


###  http://sawgraph.spatialai.org/v1/me-egad#samplePointType.srb
me_egad:samplePointType.srb rdf:type owl:NamedIndividual ,
                                     me_egad:EGAD-SamplePointType ;
                            rdfs:label "STREAM/RIVER BIOMONITORING" .


###  http://sawgraph.spatialai.org/v1/me-egad#samplePointType.ss
me_egad:samplePointType.ss rdf:type owl:NamedIndividual ,
                                    me_egad:EGAD-SamplePointType ;
                           rdfs:label "SURFACE SOIL" .


###  http://sawgraph.spatialai.org/v1/me-egad#samplePointType.st
me_egad:samplePointType.st rdf:type owl:NamedIndividual ,
                                    me_egad:EGAD-SamplePointType ;
                           rdfs:label "STREAM" .


###  http://sawgraph.spatialai.org/v1/me-egad#samplePointType.stw
me_egad:samplePointType.stw rdf:type owl:NamedIndividual ,
                                     me_egad:EGAD-SamplePointType ;
                            rdfs:label "STILLING WELL" .


###  http://sawgraph.spatialai.org/v1/me-egad#samplePointType.sw
me_egad:samplePointType.sw rdf:type owl:NamedIndividual ,
                                    me_egad:EGAD-SamplePointType ;
                           rdfs:label "STANDING WATER (E.G. PUDDLE)" .


###  http://sawgraph.spatialai.org/v1/me-egad#samplePointType.tb
me_egad:samplePointType.tb rdf:type owl:NamedIndividual ,
                                    me_egad:EGAD-SamplePointType ;
                           rdfs:label "TEST BORING" .


###  http://sawgraph.spatialai.org/v1/me-egad#samplePointType.tp
me_egad:samplePointType.tp rdf:type owl:NamedIndividual ,
                                    me_egad:EGAD-SamplePointType ;
                           rdfs:label "TEST PIT" .


###  http://sawgraph.spatialai.org/v1/me-egad#samplePointType.ts
me_egad:samplePointType.ts rdf:type owl:NamedIndividual ,
                                    me_egad:EGAD-SamplePointType ;
                           rdfs:label "TREATMENT SYSTEM" .


###  http://sawgraph.spatialai.org/v1/me-egad#samplePointType.ud
me_egad:samplePointType.ud rdf:type owl:NamedIndividual ,
                                    me_egad:EGAD-SamplePointType ;
                           rdfs:label "UNDER DRAIN" .


###  http://sawgraph.spatialai.org/v1/me-egad#samplePointType.unk
me_egad:samplePointType.unk rdf:type owl:NamedIndividual ,
                                     me_egad:EGAD-SamplePointType ;
                            rdfs:label "UNKNOWN" .


###  http://sawgraph.spatialai.org/v1/me-egad#samplePointType.ust
me_egad:samplePointType.ust rdf:type owl:NamedIndividual ,
                                     me_egad:EGAD-SamplePointType ;
                            rdfs:label "UNDERGROUND STORAGE TANK" .


###  http://sawgraph.spatialai.org/v1/me-egad#samplePointType.vms
me_egad:samplePointType.vms rdf:type owl:NamedIndividual ,
                                     me_egad:EGAD-SamplePointType ;
                            rdfs:label "VAPOR MITIGATION SYSTEM" .


###  http://sawgraph.spatialai.org/v1/me-egad#samplePointType.wd
me_egad:samplePointType.wd rdf:type owl:NamedIndividual ,
                                    me_egad:EGAD-SamplePointType ;
                           rdfs:label "WICK DRAIN" .


###  http://sawgraph.spatialai.org/v1/me-egad#samplePointType.wi
me_egad:samplePointType.wi rdf:type owl:NamedIndividual ,
                                    me_egad:EGAD-SamplePointType ;
                           rdfs:label "WILDERNESS" .


###  http://sawgraph.spatialai.org/v1/me-egad#samplePointType.wld
me_egad:samplePointType.wld rdf:type owl:NamedIndividual ,
                                     me_egad:EGAD-SamplePointType ;
                            rdfs:label "WETLAND" .


###  http://sawgraph.spatialai.org/v1/me-egad#samplePointType.wp
me_egad:samplePointType.wp rdf:type owl:NamedIndividual ,
                                    me_egad:EGAD-SamplePointType ;
                           rdfs:label "WASTE PILE" .


###  http://sawgraph.spatialai.org/v1/me-egad#sampleType.a
me_egad:sampleType.a rdf:type owl:NamedIndividual ,
                              me_egad:EGAD-SampleMaterialType ;
                     rdfs:label "AIR" .


###  http://sawgraph.spatialai.org/v1/me-egad#sampleType.al
me_egad:sampleType.al rdf:type owl:NamedIndividual ,
                               me_egad:EGAD-SampleMaterialType ;
                      rdfs:label "ALGAE" .


###  http://sawgraph.spatialai.org/v1/me-egad#sampleType.aq
me_egad:sampleType.aq rdf:type owl:NamedIndividual ,
                               me_egad:EGAD-SampleMaterialType ;
                      rdfs:label "AQUEOUS (FOR QC DATA ONLY)" .


###  http://sawgraph.spatialai.org/v1/me-egad#sampleType.as
me_egad:sampleType.as rdf:type owl:NamedIndividual ,
                               me_egad:EGAD-SampleMaterialType ;
                      rdfs:label "ASH (BOTTOM & FLY)" .


###  http://sawgraph.spatialai.org/v1/me-egad#sampleType.asp
me_egad:sampleType.asp rdf:type owl:NamedIndividual ,
                                me_egad:EGAD-SampleMaterialType ;
                       rdfs:label "ASPHALT" .


###  http://sawgraph.spatialai.org/v1/me-egad#sampleType.at
me_egad:sampleType.at rdf:type owl:NamedIndividual ,
                               me_egad:EGAD-SampleMaterialType ;
                      rdfs:label "AQUIFER TEST" .


###  http://sawgraph.spatialai.org/v1/me-egad#sampleType.ba
me_egad:sampleType.ba rdf:type owl:NamedIndividual ,
                               me_egad:EGAD-SampleMaterialType ;
                      rdfs:label "BOTTOM ASH" .


###  http://sawgraph.spatialai.org/v1/me-egad#sampleType.bc
me_egad:sampleType.bc rdf:type owl:NamedIndividual ,
                               me_egad:EGAD-SampleMaterialType ;
                      rdfs:label "BEDROCK CHIPS" .


###  http://sawgraph.spatialai.org/v1/me-egad#sampleType.bd
me_egad:sampleType.bd rdf:type owl:NamedIndividual ,
                               me_egad:EGAD-SampleMaterialType ;
                      rdfs:label "BLOOD" .


###  http://sawgraph.spatialai.org/v1/me-egad#sampleType.bm
me_egad:sampleType.bm rdf:type owl:NamedIndividual ,
                               me_egad:EGAD-SampleMaterialType ;
                      rdfs:label "BUILDING MATERIAL" .


###  http://sawgraph.spatialai.org/v1/me-egad#sampleType.car
me_egad:sampleType.car rdf:type owl:NamedIndividual ,
                                me_egad:EGAD-SampleMaterialType ;
                       rdfs:label "CARCASS" .


###  http://sawgraph.spatialai.org/v1/me-egad#sampleType.ch
me_egad:sampleType.ch rdf:type owl:NamedIndividual ,
                               me_egad:EGAD-SampleMaterialType ;
                      rdfs:label "CHEESE" .


###  http://sawgraph.spatialai.org/v1/me-egad#sampleType.co
me_egad:sampleType.co rdf:type owl:NamedIndividual ,
                               me_egad:EGAD-SampleMaterialType ;
                      rdfs:label "COMPOST" .


###  http://sawgraph.spatialai.org/v1/me-egad#sampleType.con
me_egad:sampleType.con rdf:type owl:NamedIndividual ,
                                me_egad:EGAD-SampleMaterialType ;
                       rdfs:label "CONDENSATE" .


###  http://sawgraph.spatialai.org/v1/me-egad#sampleType.cp
me_egad:sampleType.cp rdf:type owl:NamedIndividual ,
                               me_egad:EGAD-SampleMaterialType ;
                      rdfs:label "CELLULOSE PULP" .


###  http://sawgraph.spatialai.org/v1/me-egad#sampleType.ea
me_egad:sampleType.ea rdf:type owl:NamedIndividual ,
                               me_egad:EGAD-SampleMaterialType ;
                      rdfs:label "EPIPHYTIC ALGAE" .


###  http://sawgraph.spatialai.org/v1/me-egad#sampleType.eg
me_egad:sampleType.eg rdf:type owl:NamedIndividual ,
                               me_egad:EGAD-SampleMaterialType ;
                      rdfs:label "EGG" .


###  http://sawgraph.spatialai.org/v1/me-egad#sampleType.fa
me_egad:sampleType.fa rdf:type owl:NamedIndividual ,
                               me_egad:EGAD-SampleMaterialType ;
                      rdfs:label "FLY ASH" .


###  http://sawgraph.spatialai.org/v1/me-egad#sampleType.fbq
me_egad:sampleType.fbq rdf:type owl:NamedIndividual ,
                                me_egad:EGAD-SampleMaterialType ;
                       rdfs:label "FILM BRIQUETTE" .


###  http://sawgraph.spatialai.org/v1/me-egad#sampleType.fe
me_egad:sampleType.fe rdf:type owl:NamedIndividual ,
                               me_egad:EGAD-SampleMaterialType ;
                      rdfs:label "FEED" .


###  http://sawgraph.spatialai.org/v1/me-egad#sampleType.fhtw
me_egad:sampleType.fhtw rdf:type owl:NamedIndividual ,
                                 me_egad:EGAD-SampleMaterialType ;
                        rdfs:label "FISH HATCHERY TANK WATER" .


###  http://sawgraph.spatialai.org/v1/me-egad#sampleType.fi
me_egad:sampleType.fi rdf:type owl:NamedIndividual ,
                               me_egad:EGAD-SampleMaterialType ;
                      rdfs:label "FILTER" .


###  http://sawgraph.spatialai.org/v1/me-egad#sampleType.fp
me_egad:sampleType.fp rdf:type owl:NamedIndividual ,
                               me_egad:EGAD-SampleMaterialType ;
                      rdfs:label "FREE PRODUCT (FOR QC DATA ONLY)" .


###  http://sawgraph.spatialai.org/v1/me-egad#sampleType.fr
me_egad:sampleType.fr rdf:type owl:NamedIndividual ,
                               me_egad:EGAD-SampleMaterialType ;
                      rdfs:label "FRUIT" .


###  http://sawgraph.spatialai.org/v1/me-egad#sampleType.fs
me_egad:sampleType.fs rdf:type owl:NamedIndividual ,
                               me_egad:EGAD-SampleMaterialType ;
                      rdfs:label "FISH (COUNTS)" .


###  http://sawgraph.spatialai.org/v1/me-egad#sampleType.g
me_egad:sampleType.g rdf:type owl:NamedIndividual ,
                              me_egad:EGAD-SampleMaterialType ;
                     rdfs:label "GONAD" .


###  http://sawgraph.spatialai.org/v1/me-egad#sampleType.gr
me_egad:sampleType.gr rdf:type owl:NamedIndividual ,
                               me_egad:EGAD-SampleMaterialType ;
                      rdfs:label "GRAINS (GROWN BY FARM)" .


###  http://sawgraph.spatialai.org/v1/me-egad#sampleType.grs
me_egad:sampleType.grs rdf:type owl:NamedIndividual ,
                                me_egad:EGAD-SampleMaterialType ;
                       rdfs:label "GRASS" .


###  http://sawgraph.spatialai.org/v1/me-egad#sampleType.gs
me_egad:sampleType.gs rdf:type owl:NamedIndividual ,
                               me_egad:EGAD-SampleMaterialType ;
                      rdfs:label "SOIL GAS" .


###  http://sawgraph.spatialai.org/v1/me-egad#sampleType.gw
me_egad:sampleType.gw rdf:type owl:NamedIndividual ,
                               me_egad:EGAD-SampleMaterialType ;
                      rdfs:label "GROUNDWATER" .


###  http://sawgraph.spatialai.org/v1/me-egad#sampleType.gz
me_egad:sampleType.gz rdf:type owl:NamedIndividual ,
                               me_egad:EGAD-SampleMaterialType ;
                      rdfs:label "GIZZARD" .


###  http://sawgraph.spatialai.org/v1/me-egad#sampleType.hm
me_egad:sampleType.hm rdf:type owl:NamedIndividual ,
                               me_egad:EGAD-SampleMaterialType ;
                      rdfs:label "HEMP" .


###  http://sawgraph.spatialai.org/v1/me-egad#sampleType.hn
me_egad:sampleType.hn rdf:type owl:NamedIndividual ,
                               me_egad:EGAD-SampleMaterialType ;
                      rdfs:label "HONEY" .


###  http://sawgraph.spatialai.org/v1/me-egad#sampleType.hp
me_egad:sampleType.hp rdf:type owl:NamedIndividual ,
                               me_egad:EGAD-SampleMaterialType ;
                      rdfs:label "HEPATOPANCREAS (TOMALLEY)" .


###  http://sawgraph.spatialai.org/v1/me-egad#sampleType.hr
me_egad:sampleType.hr rdf:type owl:NamedIndividual ,
                               me_egad:EGAD-SampleMaterialType ;
                      rdfs:label "HERBS" .


###  http://sawgraph.spatialai.org/v1/me-egad#sampleType.hsg
me_egad:sampleType.hsg rdf:type owl:NamedIndividual ,
                                me_egad:EGAD-SampleMaterialType ;
                       rdfs:label "HEAD SPACE GAS" .


###  http://sawgraph.spatialai.org/v1/me-egad#sampleType.ht
me_egad:sampleType.ht rdf:type owl:NamedIndividual ,
                               me_egad:EGAD-SampleMaterialType ;
                      rdfs:label "HEART" .


###  http://sawgraph.spatialai.org/v1/me-egad#sampleType.ia
me_egad:sampleType.ia rdf:type owl:NamedIndividual ,
                               me_egad:EGAD-SampleMaterialType ;
                      rdfs:label "INDOOR AIR" .


###  http://sawgraph.spatialai.org/v1/me-egad#sampleType.kd
me_egad:sampleType.kd rdf:type owl:NamedIndividual ,
                               me_egad:EGAD-SampleMaterialType ;
                      rdfs:label "KIDNEY" .


###  http://sawgraph.spatialai.org/v1/me-egad#sampleType.l
me_egad:sampleType.l rdf:type owl:NamedIndividual ,
                              me_egad:EGAD-SampleMaterialType ;
                     rdfs:label "LEACHATE" .


###  http://sawgraph.spatialai.org/v1/me-egad#sampleType.ld
me_egad:sampleType.ld rdf:type owl:NamedIndividual ,
                               me_egad:EGAD-SampleMaterialType ;
                      rdfs:label "LEAK DETECTION FLUIDS" .


###  http://sawgraph.spatialai.org/v1/me-egad#sampleType.lfg
me_egad:sampleType.lfg rdf:type owl:NamedIndividual ,
                                me_egad:EGAD-SampleMaterialType ;
                       rdfs:label "LANDFILL GAS" .


###  http://sawgraph.spatialai.org/v1/me-egad#sampleType.lg
me_egad:sampleType.lg rdf:type owl:NamedIndividual ,
                               me_egad:EGAD-SampleMaterialType ;
                      rdfs:label "LEAFY GREENS" .


###  http://sawgraph.spatialai.org/v1/me-egad#sampleType.lqc
me_egad:sampleType.lqc rdf:type owl:NamedIndividual ,
                                me_egad:EGAD-SampleMaterialType ;
                       rdfs:label "LIQUID CONDENSATE" .


###  http://sawgraph.spatialai.org/v1/me-egad#sampleType.lv
me_egad:sampleType.lv rdf:type owl:NamedIndividual ,
                               me_egad:EGAD-SampleMaterialType ;
                      rdfs:label "LIVER" .


###  http://sawgraph.spatialai.org/v1/me-egad#sampleType.ma
me_egad:sampleType.ma rdf:type owl:NamedIndividual ,
                               me_egad:EGAD-SampleMaterialType ;
                      rdfs:label "MANURE" .


###  http://sawgraph.spatialai.org/v1/me-egad#sampleType.mc
me_egad:sampleType.mc rdf:type owl:NamedIndividual ,
                               me_egad:EGAD-SampleMaterialType ;
                      rdfs:label "MINERAL CRUST" .


###  http://sawgraph.spatialai.org/v1/me-egad#sampleType.mea
me_egad:sampleType.mea rdf:type owl:NamedIndividual ,
                                me_egad:EGAD-SampleMaterialType ;
                       rdfs:label "MEAT" .


###  http://sawgraph.spatialai.org/v1/me-egad#sampleType.mi
me_egad:sampleType.mi rdf:type owl:NamedIndividual ,
                               me_egad:EGAD-SampleMaterialType ;
                      rdfs:label "MACROINVERTEBRATE" .


###  http://sawgraph.spatialai.org/v1/me-egad#sampleType.mlk
me_egad:sampleType.mlk rdf:type owl:NamedIndividual ,
                                me_egad:EGAD-SampleMaterialType ;
                       rdfs:label "MILK" .


###  http://sawgraph.spatialai.org/v1/me-egad#sampleType.mps
me_egad:sampleType.mps rdf:type owl:NamedIndividual ,
                                me_egad:EGAD-SampleMaterialType ;
                       rdfs:label "MAPLE SYRUP" .


###  http://sawgraph.spatialai.org/v1/me-egad#sampleType.mr
me_egad:sampleType.mr rdf:type owl:NamedIndividual ,
                               me_egad:EGAD-SampleMaterialType ;
                      rdfs:label "MUSHROOM" .


###  http://sawgraph.spatialai.org/v1/me-egad#sampleType.mtb
me_egad:sampleType.mtb rdf:type owl:NamedIndividual ,
                                me_egad:EGAD-SampleMaterialType ;
                       rdfs:label "MUSCLE TISSUE BIOPSY" .


###  http://sawgraph.spatialai.org/v1/me-egad#sampleType.mu
me_egad:sampleType.mu rdf:type owl:NamedIndividual ,
                               me_egad:EGAD-SampleMaterialType ;
                      rdfs:label "MUSCLE" .


###  http://sawgraph.spatialai.org/v1/me-egad#sampleType.n
me_egad:sampleType.n rdf:type owl:NamedIndividual ,
                              me_egad:EGAD-SampleMaterialType ;
                     rdfs:label "NEAT SAMPLE" .


###  http://sawgraph.spatialai.org/v1/me-egad#sampleType.no
me_egad:sampleType.no rdf:type owl:NamedIndividual ,
                               me_egad:EGAD-SampleMaterialType ;
                      rdfs:label "NOTIFICATION" .


###  http://sawgraph.spatialai.org/v1/me-egad#sampleType.nrv
me_egad:sampleType.nrv rdf:type owl:NamedIndividual ,
                                me_egad:EGAD-SampleMaterialType ;
                       rdfs:label "NON-ROOT VEGETABLES" .


###  http://sawgraph.spatialai.org/v1/me-egad#sampleType.o
me_egad:sampleType.o rdf:type owl:NamedIndividual ,
                              me_egad:EGAD-SampleMaterialType ;
                     rdfs:label "OFFAL" .


###  http://sawgraph.spatialai.org/v1/me-egad#sampleType.oa
me_egad:sampleType.oa rdf:type owl:NamedIndividual ,
                               me_egad:EGAD-SampleMaterialType ;
                      rdfs:label "OUTDOOR AIR" .


###  http://sawgraph.spatialai.org/v1/me-egad#sampleType.pc
me_egad:sampleType.pc rdf:type owl:NamedIndividual ,
                               me_egad:EGAD-SampleMaterialType ;
                      rdfs:label "PHYSICAL CHARACTERISTIC" .


###  http://sawgraph.spatialai.org/v1/me-egad#sampleType.pe
me_egad:sampleType.pe rdf:type owl:NamedIndividual ,
                               me_egad:EGAD-SampleMaterialType ;
                      rdfs:label "PERFORMANCE EVALUATION" .


###  http://sawgraph.spatialai.org/v1/me-egad#sampleType.po
me_egad:sampleType.po rdf:type owl:NamedIndividual ,
                               me_egad:EGAD-SampleMaterialType ;
                      rdfs:label "PORE WATER" .


###  http://sawgraph.spatialai.org/v1/me-egad#sampleType.pol
me_egad:sampleType.pol rdf:type owl:NamedIndividual ,
                                me_egad:EGAD-SampleMaterialType ;
                       rdfs:label "POLYMER" .


###  http://sawgraph.spatialai.org/v1/me-egad#sampleType.pp
me_egad:sampleType.pp rdf:type owl:NamedIndividual ,
                               me_egad:EGAD-SampleMaterialType ;
                      rdfs:label "PHYTOPLANKTON" .


###  http://sawgraph.spatialai.org/v1/me-egad#sampleType.pr
me_egad:sampleType.pr rdf:type owl:NamedIndividual ,
                               me_egad:EGAD-SampleMaterialType ;
                      rdfs:label "PRECIPITATION" .


###  http://sawgraph.spatialai.org/v1/me-egad#sampleType.pw
me_egad:sampleType.pw rdf:type owl:NamedIndividual ,
                               me_egad:EGAD-SampleMaterialType ;
                      rdfs:label "PROCESS WATER" .


###  http://sawgraph.spatialai.org/v1/me-egad#sampleType.rn
me_egad:sampleType.rn rdf:type owl:NamedIndividual ,
                               me_egad:EGAD-SampleMaterialType ;
                      rdfs:label "RAIN PRECIPITATION" .


###  http://sawgraph.spatialai.org/v1/me-egad#sampleType.rv
me_egad:sampleType.rv rdf:type owl:NamedIndividual ,
                               me_egad:EGAD-SampleMaterialType ;
                      rdfs:label "ROOT VEGETABLES" .


###  http://sawgraph.spatialai.org/v1/me-egad#sampleType.sa
me_egad:sampleType.sa rdf:type owl:NamedIndividual ,
                               me_egad:EGAD-SampleMaterialType ;
                      rdfs:label "SAWDUST" .


###  http://sawgraph.spatialai.org/v1/me-egad#sampleType.sd
me_egad:sampleType.sd rdf:type owl:NamedIndividual ,
                               me_egad:EGAD-SampleMaterialType ;
                      rdfs:label "SEDIMENT" .


###  http://sawgraph.spatialai.org/v1/me-egad#sampleType.sf
me_egad:sampleType.sf rdf:type owl:NamedIndividual ,
                               me_egad:EGAD-SampleMaterialType ;
                      rdfs:label "SKINLESS FILLET" .


###  http://sawgraph.spatialai.org/v1/me-egad#sampleType.sk
me_egad:sampleType.sk rdf:type owl:NamedIndividual ,
                               me_egad:EGAD-SampleMaterialType ;
                      rdfs:label "SKIN" .


###  http://sawgraph.spatialai.org/v1/me-egad#sampleType.sl
me_egad:sampleType.sl rdf:type owl:NamedIndividual ,
                               me_egad:EGAD-SampleMaterialType ;
                      rdfs:label "SOIL" .


###  http://sawgraph.spatialai.org/v1/me-egad#sampleType.sld
me_egad:sampleType.sld rdf:type owl:NamedIndividual ,
                                me_egad:EGAD-SampleMaterialType ;
                       rdfs:label "SOLID (FOR QC DATA ONLY)" .


###  http://sawgraph.spatialai.org/v1/me-egad#sampleType.snw
me_egad:sampleType.snw rdf:type owl:NamedIndividual ,
                                me_egad:EGAD-SampleMaterialType ;
                       rdfs:label "SNOW PRECIPITATION" .


###  http://sawgraph.spatialai.org/v1/me-egad#sampleType.sof
me_egad:sampleType.sof rdf:type owl:NamedIndividual ,
                                me_egad:EGAD-SampleMaterialType ;
                       rdfs:label "SKIN-ON FILLET" .


###  http://sawgraph.spatialai.org/v1/me-egad#sampleType.spg
me_egad:sampleType.spg rdf:type owl:NamedIndividual ,
                                me_egad:EGAD-SampleMaterialType ;
                       rdfs:label "SEPTAGE" .


###  http://sawgraph.spatialai.org/v1/me-egad#sampleType.sr
me_egad:sampleType.sr rdf:type owl:NamedIndividual ,
                               me_egad:EGAD-SampleMaterialType ;
                      rdfs:label "STORM WATER RUNOFF" .


###  http://sawgraph.spatialai.org/v1/me-egad#sampleType.ssg
me_egad:sampleType.ssg rdf:type owl:NamedIndividual ,
                                me_egad:EGAD-SampleMaterialType ;
                       rdfs:label "SUBSLAB GAS" .


###  http://sawgraph.spatialai.org/v1/me-egad#sampleType.su
me_egad:sampleType.su rdf:type owl:NamedIndividual ,
                               me_egad:EGAD-SampleMaterialType ;
                      rdfs:label "SLUDGE" .


###  http://sawgraph.spatialai.org/v1/me-egad#sampleType.sul
me_egad:sampleType.sul rdf:type owl:NamedIndividual ,
                                me_egad:EGAD-SampleMaterialType ;
                       rdfs:label "SLUDGE - LIMED" .


###  http://sawgraph.spatialai.org/v1/me-egad#sampleType.suu
me_egad:sampleType.suu rdf:type owl:NamedIndividual ,
                                me_egad:EGAD-SampleMaterialType ;
                       rdfs:label "SLUDGE - UNLIMED" .


###  http://sawgraph.spatialai.org/v1/me-egad#sampleType.sw
me_egad:sampleType.sw rdf:type owl:NamedIndividual ,
                               me_egad:EGAD-SampleMaterialType ;
                      rdfs:label "SURFACE WATER" .


###  http://sawgraph.spatialai.org/v1/me-egad#sampleType.sws
me_egad:sampleType.sws rdf:type owl:NamedIndividual ,
                                me_egad:EGAD-SampleMaterialType ;
                       rdfs:label "SURFACE WATER SUBSTRATE" .


###  http://sawgraph.spatialai.org/v1/me-egad#sampleType.to
me_egad:sampleType.to rdf:type owl:NamedIndividual ,
                               me_egad:EGAD-SampleMaterialType ;
                      rdfs:label "TONGUE" .


###  http://sawgraph.spatialai.org/v1/me-egad#sampleType.ts
me_egad:sampleType.ts rdf:type owl:NamedIndividual ,
                               me_egad:EGAD-SampleMaterialType ;
                      rdfs:label "TISSUE (FOR QC DATA ONLY)" .


###  http://sawgraph.spatialai.org/v1/me-egad#sampleType.u
me_egad:sampleType.u rdf:type owl:NamedIndividual ,
                              me_egad:EGAD-SampleMaterialType ;
                     rdfs:label "UNKNOWN" .


###  http://sawgraph.spatialai.org/v1/me-egad#sampleType.v
me_egad:sampleType.v rdf:type owl:NamedIndividual ,
                              me_egad:EGAD-SampleMaterialType ;
                     rdfs:label "VEGETATION" .


###  http://sawgraph.spatialai.org/v1/me-egad#sampleType.w
me_egad:sampleType.w rdf:type owl:NamedIndividual ,
                              me_egad:EGAD-SampleMaterialType ;
                     rdfs:label "WASTE" .


###  http://sawgraph.spatialai.org/v1/me-egad#sampleType.wc
me_egad:sampleType.wc rdf:type owl:NamedIndividual ,
                               me_egad:EGAD-SampleMaterialType ;
                      rdfs:label "WOOD CHIPS" .


###  http://sawgraph.spatialai.org/v1/me-egad#sampleType.wh
me_egad:sampleType.wh rdf:type owl:NamedIndividual ,
                               me_egad:EGAD-SampleMaterialType ;
                      rdfs:label "WHOLE" .


###  http://sawgraph.spatialai.org/v1/me-egad#sampleType.wp
me_egad:sampleType.wp rdf:type owl:NamedIndividual ,
                               me_egad:EGAD-SampleMaterialType ;
                      rdfs:label "WIPE" .


###  http://sawgraph.spatialai.org/v1/me-egad#sampleType.ws
me_egad:sampleType.ws rdf:type owl:NamedIndividual ,
                               me_egad:EGAD-SampleMaterialType ;
                      rdfs:label "WHOLE WITHOUT SKIN" .


###  http://sawgraph.spatialai.org/v1/me-egad#sampleType.ww
me_egad:sampleType.ww rdf:type owl:NamedIndividual ,
                               me_egad:EGAD-SampleMaterialType ;
                      rdfs:label "WASTE WATER" .


###  http://sawgraph.spatialai.org/v1/me-egad#sampleType.wwhg
me_egad:sampleType.wwhg rdf:type owl:NamedIndividual ,
                                 me_egad:EGAD-SampleMaterialType ;
                        rdfs:label "WHOLE WITHOUT HEAD OR GUT" .


###  http://sawgraph.spatialai.org/v1/me-egad#siteType.agric-chem
me_egad:siteType.agric-chem rdf:type owl:NamedIndividual ,
                                     me_egad:EGAD-SiteType ;
                            rdfs:comment "An area of large commercial farming and orchards that appear on field inspection to have pesticide use. Evidence includes tractors with spray bars, totally weed-free crops, etc. Also includes large farm supply stores noted during watershed inspections." ;
                            rdfs:label "AGRICULTURAL CHEMICAL USE" .


###  http://sawgraph.spatialai.org/v1/me-egad#siteType.agric-farm
me_egad:siteType.agric-farm rdf:type owl:NamedIndividual ,
                                     me_egad:EGAD-SiteType ;
                            rdfs:comment "Includes dairies, feedlots, large herds of livestock, and chicken farms, as well as areas with recent sludge spreading as part of the Statewide PFAS Investigation under Maine LD 1600." ;
                            rdfs:label "AGRICULTURAL FARM PRODUCTS" .


###  http://sawgraph.spatialai.org/v1/me-egad#siteType.agric-nitr_bac
me_egad:siteType.agric-nitr_bac rdf:type owl:NamedIndividual ,
                                         me_egad:EGAD-SiteType ;
                                rdfs:comment "Includes dairies, feedlots, large herds of livestock, and chicken farms, as well as areas with recent manure spreading noted during watershed inspections." ;
                                rdfs:label "AGRICULTURE NITRATE/BACTERIA" .


###  http://sawgraph.spatialai.org/v1/me-egad#siteType.aqua
me_egad:siteType.aqua rdf:type owl:NamedIndividual ,
                               me_egad:EGAD-SiteType ;
                      rdfs:comment "A facility for farming aquatic species." ;
                      rdfs:label "AQUACULTURE" .


###  http://sawgraph.spatialai.org/v1/me-egad#siteType.ash-util
me_egad:siteType.ash-util rdf:type owl:NamedIndividual ,
                                   me_egad:EGAD-SiteType ;
                          rdfs:comment "A site at which the residue (biomass ash) remaining after the combustion of tree parts, paper mill sludge, wood from demolition debris, peat, or the combustion of wood with fossil fuels or other material has been spread on the land." ;
                          rdfs:label "ASH UTILIZATION SITE" .


###  http://sawgraph.spatialai.org/v1/me-egad#siteType.auto-junk
me_egad:siteType.auto-junk rdf:type owl:NamedIndividual ,
                                    me_egad:EGAD-SiteType ;
                           rdfs:comment "An area used to store three or more unserviceable, discarded, worn out or junked motor vehicles. Also includes an area used for automobile dismantling, salvage and recycling operations." ;
                           rdfs:label "AUTOMOBILE GRAVEYARD/JUNKYARD" .


###  http://sawgraph.spatialai.org/v1/me-egad#siteType.ben-reuse
me_egad:siteType.ben-reuse rdf:type owl:NamedIndividual ,
                                    me_egad:EGAD-SiteType ;
                           rdfs:comment "A site involved in the use or reuse of a solid waste or waste derived product." ;
                           rdfs:label "BENEFICIAL REUSE" .


###  http://sawgraph.spatialai.org/v1/me-egad#siteType.bk-study
me_egad:siteType.bk-study rdf:type owl:NamedIndividual ,
                                   me_egad:EGAD-SiteType ;
                          rdfs:comment "A site used for determination of background contamination concentrations." ;
                          rdfs:label "BACKGROUND STUDY SITE" .


###  http://sawgraph.spatialai.org/v1/me-egad#siteType.brownfields
me_egad:siteType.brownfields rdf:type owl:NamedIndividual ,
                                      me_egad:EGAD-SiteType ;
                             rdfs:comment "Site that receives federal or state funding or services under the Brownfields Program for a property where redevelopment is impeded by the presence or potential presence of contaminants." ;
                             rdfs:label "BROWNFIELDS" .


###  http://sawgraph.spatialai.org/v1/me-egad#siteType.comp
me_egad:siteType.comp rdf:type owl:NamedIndividual ,
                               me_egad:EGAD-SiteType ;
                      rdfs:comment "A site at which compost is produced. Compost is the humus-like product resulting from the biological decomposition of organic matter under aerobic conditions at high temperature. This material may be used as a soil amendment." ;
                      rdfs:label "COMPOST SITE" .


###  http://sawgraph.spatialai.org/v1/me-egad#siteType.con_dem
me_egad:siteType.con_dem rdf:type owl:NamedIndividual ,
                                  me_egad:EGAD-SiteType ;
                         rdfs:comment "A site at which debris resulting from construction, remodeling, repair, and demolition of structures have been disposed. It excludes asbestos and other special wastes." ;
                         rdfs:label "CONSTRUCTION/DEMOLITION SITE" .


###  http://sawgraph.spatialai.org/v1/me-egad#siteType.dmp
me_egad:siteType.dmp rdf:type owl:NamedIndividual ,
                              me_egad:EGAD-SiteType ;
                     rdfs:comment "Sites at which organisms (predominantly fish, occasionally shellfish) and sediments are monitored for contamination with the chemicals dioxins/furans." ;
                     rdfs:label "DIOXIN MONITORING PROGRAM" .


###  http://sawgraph.spatialai.org/v1/me-egad#siteType.dry-cln
me_egad:siteType.dry-cln rdf:type owl:NamedIndividual ,
                                  me_egad:EGAD-SiteType ;
                         rdfs:comment "A former or current location of a dry cleaners which is currently using or historically used perchloroethylene (PCE)." ;
                         rdfs:label "DRY CLEANER" .


###  http://sawgraph.spatialai.org/v1/me-egad#siteType.e-waste-coll
me_egad:siteType.e-waste-coll rdf:type owl:NamedIndividual ,
                                       me_egad:EGAD-SiteType ;
                              rdfs:comment "Any type of electronic waste (E-Waste) storage facility, including consolidators, generator-owned central accumulators, or municipal transfer stations or recycling centers." ;
                              rdfs:label "E-WASTE COLLECTION" .


###  http://sawgraph.spatialai.org/v1/me-egad#siteType.eng-swds
me_egad:siteType.eng-swds rdf:type owl:NamedIndividual ,
                                   me_egad:EGAD-SiteType ;
                          rdfs:comment "A system which is designed to infiltrate flows of greater than 2000 gallons per day into the ground." ;
                          rdfs:label "ENGINEERED SUBSURFACE WASTEWATER DISPOSAL SYSTEM" .


###  http://sawgraph.spatialai.org/v1/me-egad#siteType.estuarine
me_egad:siteType.estuarine rdf:type owl:NamedIndividual ,
                                    me_egad:EGAD-SiteType ;
                           rdfs:comment "A site in an estuary (semi-enclosed coastal water with a free connection with the open sea, and salinity typically 0.5 to 25 parts per thousand) where monitoring or assessment activities for water or sediment quality, habitat condition, and/or biological purposes." ;
                           rdfs:label "ESTUARINE" .


###  http://sawgraph.spatialai.org/v1/me-egad#siteType.fish-hatchery
me_egad:siteType.fish-hatchery rdf:type owl:NamedIndividual ,
                                        me_egad:EGAD-SiteType ;
                               rdfs:comment "A facility for the breeding and rearing of fish species." ;
                               rdfs:label "FISH HATCHERY" .


###  http://sawgraph.spatialai.org/v1/me-egad#siteType.ind-compl
me_egad:siteType.ind-compl rdf:type owl:NamedIndividual ,
                                    me_egad:EGAD-SiteType ;
                           rdfs:comment "A non-point source site where manufactured goods are produced.  Runoff and infiltration of water from these sites may carry substances which can contaminate ground water." ;
                           rdfs:label "INDUSTRIAL COMPLEX" .


###  http://sawgraph.spatialai.org/v1/me-egad#siteType.inf_ret-bas
me_egad:siteType.inf_ret-bas rdf:type owl:NamedIndividual ,
                                      me_egad:EGAD-SiteType ;
                             rdfs:comment "A site at which run-off or other surface flow enters a property other than where it originated, and where water is held while it slowly penetrates through the ground surface into the subsurface soil." ;
                             rdfs:label "INFILTRATION/RETENTION BASIN" .


###  http://sawgraph.spatialai.org/v1/me-egad#siteType.lake-pond
me_egad:siteType.lake-pond rdf:type owl:NamedIndividual ,
                                    me_egad:EGAD-SiteType ;
                           rdfs:comment "A body of (usually fresh) lentic water surrounded by land where monitoring or assessment activities for quality of water, sediment, habitat, and/or biolgoical communities occur. Includes lake and pond ecosystems." ;
                           rdfs:label "LAKE/POND" .


###  http://sawgraph.spatialai.org/v1/me-egad#siteType.last
me_egad:siteType.last rdf:type owl:NamedIndividual ,
                               me_egad:EGAD-SiteType ;
                      rdfs:comment "(LAST). A container, 90% or more of which is above the ground, which is used to hold oil and other petroleum derived products.  It is considered to be leaking if there is some evidence that it has released some of its contents to the environment." ;
                      rdfs:label "LEAKING ABOVEGROUND STORAGE TANK" .


###  http://sawgraph.spatialai.org/v1/me-egad#siteType.lf-com
me_egad:siteType.lf-com rdf:type owl:NamedIndividual ,
                                 me_egad:EGAD-SiteType ;
                        rdfs:comment "Commercially owned and/or operated solid waste landfill licensed to accept municipal solid waste (from household and normal commercial sources)." ;
                        rdfs:label "LANDFILL COMMERCIAL" .


###  http://sawgraph.spatialai.org/v1/me-egad#siteType.lf-mun
me_egad:siteType.lf-mun rdf:type owl:NamedIndividual ,
                                 me_egad:EGAD-SiteType ;
                        rdfs:comment "Municipally owned and operated solid landfill licensed to accept municipal solid waste (from household and normal commercial sources)." ;
                        rdfs:label "LANDFILL MUNICIPAL" .


###  http://sawgraph.spatialai.org/v1/me-egad#siteType.lf-spw
me_egad:siteType.lf-spw rdf:type owl:NamedIndividual ,
                                 me_egad:EGAD-SiteType ;
                        rdfs:comment "A landfill that accepts special solid waste (not from household or typical commercial sources, that exists in an unusual quantity/state such that it may impair effective waste management, or threaten human safety or the environment." ;
                        rdfs:label "LANDFILL SPECIAL WASTE" .


###  http://sawgraph.spatialai.org/v1/me-egad#siteType.lg-bulk-fuel
me_egad:siteType.lg-bulk-fuel rdf:type owl:NamedIndividual ,
                                       me_egad:EGAD-SiteType ;
                              rdfs:comment "A group of large above ground storage tanks (ASTs) usually used to store petroleum products, (i.e., marine terminals, petroleum distribution facilities), with a total facility volume greater than 1320 gallons (requires a Spill Prevention, Control and Countermeasure (SPCC) Plan." ;
                              rdfs:label "LARGE BULK FUEL STORAGE/DISTRIBUTION FACILITY" .


###  http://sawgraph.spatialai.org/v1/me-egad#siteType.lqg
me_egad:siteType.lqg rdf:type owl:NamedIndividual ,
                              me_egad:EGAD-SiteType ;
                     rdfs:comment "A Resource Conservation and Recovery Act (RCRA) Fully Regulated Generator that generates more than 1000 kilograms of hazardous waste per month. Hazardous waste cannot be stored more than 90 days from date of generation." ;
                     rdfs:label "RCRA LARGE QUANTITY GENERATOR" .


###  http://sawgraph.spatialai.org/v1/me-egad#siteType.lust
me_egad:siteType.lust rdf:type owl:NamedIndividual ,
                               me_egad:EGAD-SiteType ;
                      rdfs:comment "(LUST). A container, 10% or more of which is beneath the surface of the ground, which is used to hold oil and other petroleum derived products. It is considered to be leaking if there is some evidence that it has released some of its contents to the environment." ;
                      rdfs:label "LEAKING UNDERGROUND STORAGE TANK" .


###  http://sawgraph.spatialai.org/v1/me-egad#siteType.mar-boat
me_egad:siteType.mar-boat rdf:type owl:NamedIndividual ,
                                   me_egad:EGAD-SiteType ;
                          rdfs:comment "A waterfront location where large concentrations of boats are stored, fueled, repaired or constructed. Usually identified by signage during watershed inspections or from shorefront boat survey. Generally restricted to clearly commercial operations." ;
                          rdfs:label "MARINA/BOATYARD" .


###  http://sawgraph.spatialai.org/v1/me-egad#siteType.marine
me_egad:siteType.marine rdf:type owl:NamedIndividual ,
                                 me_egad:EGAD-SiteType ;
                        rdfs:comment "A marine location (with a typical salinity greater than 25 parts per thousand) where monitoring or assessment activities for water or sediment quality, habitat condition, and/or biological communities or organisms occur." ;
                        rdfs:label "MARINE" .


###  http://sawgraph.spatialai.org/v1/me-egad#siteType.mqg
me_egad:siteType.mqg rdf:type owl:NamedIndividual ,
                              me_egad:EGAD-SiteType ;
                     rdfs:comment "A Resource Conservation and Recovery Act (RCRA) generator that generates between 100 and 1000 kilograms (220-2200 lbs) of hazardous waste per month, either on average per month or exceeding 100 kg in any one month." ;
                     rdfs:label "RCRA MEDIUM QUANTITY GENERATOR" .


###  http://sawgraph.spatialai.org/v1/me-egad#siteType.myst-sp
me_egad:siteType.myst-sp rdf:type owl:NamedIndividual ,
                                  me_egad:EGAD-SiteType ;
                         rdfs:comment "A spill at which, although the contaminant is known as well as the impacted location, the source of the contaminant was unknown at the time that the data was reported." ;
                         rdfs:label "MYSTERY SPILL" .


###  http://sawgraph.spatialai.org/v1/me-egad#siteType.nps
me_egad:siteType.nps rdf:type owl:NamedIndividual ,
                              me_egad:EGAD-SiteType ;
                     rdfs:comment "Stormwater runoff from these sites may carry fertilizer, pesticides, nutrients and other compounds which may contaminate ground and surface water. Includes golfcourses, industrial complexes (incinerators, pulp and papermills, industrial parks, manufacturing." ;
                     rdfs:label "NON-POINT SOURCE" .


###  http://sawgraph.spatialai.org/v1/me-egad#siteType.rcra-rem
me_egad:siteType.rcra-rem rdf:type owl:NamedIndividual ,
                                   me_egad:EGAD-SiteType ;
                          rdfs:comment "A Resource Conservation and Recovery Act (RCRA) hazardous treatment, storage, or disposal site at which a hazardous waste generator is conducting site and groundwater remediation." ;
                          rdfs:label "RCRA REMEDIATION" .


###  http://sawgraph.spatialai.org/v1/me-egad#siteType.res-extr
me_egad:siteType.res-extr rdf:type owl:NamedIndividual ,
                                   me_egad:EGAD-SiteType ;
                          rdfs:comment "A site at which surface or underground mining has been or is being conducted. These sites may include gravel pits, above ground or underground metallic mineral mines, etc." ;
                          rdfs:label "RESOURCE EXTRACTION ACTIVITY" .


###  http://sawgraph.spatialai.org/v1/me-egad#siteType.res-extr-gw
me_egad:siteType.res-extr-gw rdf:type owl:NamedIndividual ,
                                      me_egad:EGAD-SiteType ;
                             rdfs:comment "A site where groundwater is extracted for human consumption, such as for bottling and sale on the open market, or for sale and distribution on a municipal level." ;
                             rdfs:label "RESOURCE EXTRACTION (GROUNDWATER)" .


###  http://sawgraph.spatialai.org/v1/me-egad#siteType.res-util
me_egad:siteType.res-util rdf:type owl:NamedIndividual ,
                                   me_egad:EGAD-SiteType ;
                          rdfs:comment "A site for materials that are suitable for controlled land application, resulting in vegetative assimilation, attenuation, or improved soil condition. Includes residuals from processing vegetables, fish, and other foods. (See also ash and sludge categories)." ;
                          rdfs:label "RESIDUALS UTILIZATION SITE" .


###  http://sawgraph.spatialai.org/v1/me-egad#siteType.river_stream
me_egad:siteType.river_stream rdf:type owl:NamedIndividual ,
                                       me_egad:EGAD-SiteType ;
                              rdfs:comment "A natural stream of water where monitoring or assessment activities for water or sediment quality, habitat condition, and/or biological communities or organisms take place." ;
                              rdfs:label "RIVER/STREAM" .


###  http://sawgraph.spatialai.org/v1/me-egad#siteType.s_i-wwtf
me_egad:siteType.s_i-wwtf rdf:type owl:NamedIndividual ,
                                   me_egad:EGAD-SiteType ;
                          rdfs:comment "A wastewater treatment facility (WWTF) used for treating sanitary or industrial wastewater. This may include spray irrigation sites, aerated lagoons, stabilization ponds, polishing ponds, sand filters,and other similar structures used for that purpose." ;
                          rdfs:label "SANITARY & INDUSTRIAL WWTF" .


###  http://sawgraph.spatialai.org/v1/me-egad#siteType.s_s
me_egad:siteType.s_s rdf:type owl:NamedIndividual ,
                              me_egad:EGAD-SiteType ;
                     rdfs:comment "An area at which salt, or sand-and-salt, are stored in preparation for road and highway deicing." ;
                     rdfs:label "SAND/SALT STORAGE" .


###  http://sawgraph.spatialai.org/v1/me-egad#siteType.sept-stor
me_egad:siteType.sept-stor rdf:type owl:NamedIndividual ,
                                    me_egad:EGAD-SiteType ;
                           rdfs:comment "A site on which a mixture of liquid and solid septage have been spread on the land, or where such waste is stored. Septage sources may be domestic or commercial." ;
                           rdfs:label "SEPTAGE DISPOSAL/STORAGE SITE" .


###  http://sawgraph.spatialai.org/v1/me-egad#siteType.sia
me_egad:siteType.sia rdf:type owl:NamedIndividual ,
                              me_egad:EGAD-SiteType ;
                     rdfs:comment "An unlicensed site once used for the disposal of liquid wastes." ;
                     rdfs:label "SURFACE IMPOUNDMENT ASSESSMENT SITE" .


###  http://sawgraph.spatialai.org/v1/me-egad#siteType.sl-util
me_egad:siteType.sl-util rdf:type owl:NamedIndividual ,
                                  me_egad:EGAD-SiteType ;
                         rdfs:comment "A site at which the solid, semi-solid or liquid material generated by a municipal, commercial or industrial wastewater treatment plant is spread on the land." ;
                         rdfs:label "SLUDGE UTILIZATION SITE" .


###  http://sawgraph.spatialai.org/v1/me-egad#siteType.sm-bulk-fuel
me_egad:siteType.sm-bulk-fuel rdf:type owl:NamedIndividual ,
                                       me_egad:EGAD-SiteType ;
                              rdfs:comment "A small above ground storage tank (AST) usually used to store petroleum products, with a total facility volume less than 1320 gallons. This includes marine, highway, and other commercial, private, and public entities supplied by petroleum distributors." ;
                              rdfs:label "SMALL BULK FUEL STORAGE/DISTRIBUTION FACILITY" .


###  http://sawgraph.spatialai.org/v1/me-egad#siteType.sqg
me_egad:siteType.sqg rdf:type owl:NamedIndividual ,
                              me_egad:EGAD-SiteType ;
                     rdfs:comment "A Resource Conservation and Recovery Act (RCRA) generator that generates less than 100 kilograms of hazardous waste per month AND accumulates no more than 55 gallons (1 drum; ~208 kg) of hazardous waste per month." ;
                     rdfs:label "RCRA SMALL QUANTITY GENERATOR" .


###  http://sawgraph.spatialai.org/v1/me-egad#siteType.stream-river
me_egad:siteType.stream-river rdf:type owl:NamedIndividual ,
                                       me_egad:EGAD-SiteType ;
                              rdfs:comment "A site in classified streams or rivers where monitoring or assessment activities for quality of water, sediment, habitat, and/or biological communities occur. Includes waterbodies called creek or brook." ;
                              rdfs:label "STREAM/RIVER BIOMONITORING" .


###  http://sawgraph.spatialai.org/v1/me-egad#siteType.strm-swr
me_egad:siteType.strm-swr rdf:type owl:NamedIndividual ,
                                   me_egad:EGAD-SiteType ;
                          rdfs:comment "A storm drain or sewer system designed to drain excess rain and groundwater from impervious surfaces. May include mixing of storm water and sewage." ;
                          rdfs:label "STORM SEWER" .


###  http://sawgraph.spatialai.org/v1/me-egad#siteType.surf-sp
me_egad:siteType.surf-sp rdf:type owl:NamedIndividual ,
                                  me_egad:EGAD-SiteType ;
                         rdfs:comment "A site where oil has been released onto the ground, not caused by a leak from a storage tank. Common examples include heating oil and gasoline tank overfills, tanker truck accidents and releases from gasoline tanks mounted on vehicles." ;
                         rdfs:label "SURFACE SPILL" .


###  http://sawgraph.spatialai.org/v1/me-egad#siteType.swatl
me_egad:siteType.swatl rdf:type owl:NamedIndividual ,
                                me_egad:EGAD-SiteType ;
                       rdfs:comment "Sites in lakes or ponds at which organisms (predominantly fish) and sediments are monitored for contamination with toxic chemicals such as heavy metals or polychlorinated biphenyls (PCBs)." ;
                       rdfs:label "SWAT (SURFACE WATER AMBIENT TOXICS) - LAKES" .


###  http://sawgraph.spatialai.org/v1/me-egad#siteType.swatm
me_egad:siteType.swatm rdf:type owl:NamedIndividual ,
                                me_egad:EGAD-SiteType ;
                       rdfs:comment "Sites in estuaries and near-shore marine environments at which organisms (mussels, lobster, etc.) and sediments are monitored for contamination with toxic chemicals such as heavy metals or polychlorinated biphenyls (PCBs)." ;
                       rdfs:label "SWAT (SURFACE WATER AMBIENT TOXICS) - MARINE" .


###  http://sawgraph.spatialai.org/v1/me-egad#siteType.swatrs
me_egad:siteType.swatrs rdf:type owl:NamedIndividual ,
                                 me_egad:EGAD-SiteType ;
                        rdfs:comment "Sites in rivers or streams at which organisms (predominantly fish) and sediments are monitored for contamination with toxic chemicals such as heavy metals or polychlorinated biphenyls (PCBs)." ;
                        rdfs:label "SWAT (SURFACE WATER AMBIENT TOXICS) - RIVERS & STREAMS" .


###  http://sawgraph.spatialai.org/v1/me-egad#siteType.ts
me_egad:siteType.ts rdf:type owl:NamedIndividual ,
                             me_egad:EGAD-SiteType ;
                    rdfs:comment "A waste facility constructed and managed for storage, compaction and/or placement of solid waste for movement to another waste facility." ;
                    rdfs:label "TRANSFER STATION" .


###  http://sawgraph.spatialai.org/v1/me-egad#siteType.uic
me_egad:siteType.uic rdf:type owl:NamedIndividual ,
                              me_egad:EGAD-SiteType ;
                     rdfs:comment "A site which discharges into sources of drinking water. Includes sump and separator systems discharging to wastewater disposal systems, septic systems that discharge industrial/commercial wastewater (photoprocessing, drycleaning, etc.), and dry wells." ;
                     rdfs:label "UNDERGROUND INJECTION SITE" .


###  http://sawgraph.spatialai.org/v1/me-egad#siteType.unc-dod
me_egad:siteType.unc-dod rdf:type owl:NamedIndividual ,
                                  me_egad:EGAD-SiteType ;
                         rdfs:comment "An uncontrolled hazardous substance site owned by the Department of Defense (DOD). A location at which hazardous substances came to be located, where the site poses a threat or hazard to any person or the natural environment and requires action to abate/clean." ;
                         rdfs:label "UNCONTROLLED SITE, DOD" .


###  http://sawgraph.spatialai.org/v1/me-egad#siteType.unc-npl
me_egad:siteType.unc-npl rdf:type owl:NamedIndividual ,
                                  me_egad:EGAD-SiteType ;
                         rdfs:comment "A Superfund (National Priorities List) uncontrolled hazardous substance site. A location at which hazardous substances came to be located, where the site poses a threat or hazard to any person or the natural environment and requires action to abate/clean." ;
                         rdfs:label "UNCONTROLLED SITE, NPL" .


###  http://sawgraph.spatialai.org/v1/me-egad#siteType.unc-other
me_egad:siteType.unc-other rdf:type owl:NamedIndividual ,
                                    me_egad:EGAD-SiteType ;
                           rdfs:comment "An uncontrolled hazardous substance site, not DOD or NPL (see respective categories). A location at which hazardous substances came to be located, where the site poses a threat or hazard to any person or the natural environment and requires action to abate/clean." ;
                           rdfs:label "UNCONTROLLED SITE, ALL OTHER" .


###  http://sawgraph.spatialai.org/v1/me-egad#siteType.univ-waster-hand
me_egad:siteType.univ-waster-hand rdf:type owl:NamedIndividual ,
                                           me_egad:EGAD-SiteType ;
                                  rdfs:comment "Any type of universal waste storer including a consolidator, generator-owned central accumulator, or municipal transfer station or recycling center." ;
                                  rdfs:label "UNIVERSAL WASTE HANDLER" .


###  http://sawgraph.spatialai.org/v1/me-egad#siteType.uns-sub
me_egad:siteType.uns-sub rdf:type owl:NamedIndividual ,
                                  me_egad:EGAD-SiteType ;
                         rdfs:comment "A high density commercial or residential subdivision, condominium, or trailer park which depends on individual subsurface wastewater disposal systems for the disposal of sanitary wastewater." ;
                         rdfs:label "UNSEWERED SUBDIVISION" .


###  http://sawgraph.spatialai.org/v1/me-egad#siteType.uosf
me_egad:siteType.uosf rdf:type owl:NamedIndividual ,
                               me_egad:EGAD-SiteType ;
                      rdfs:comment "Any underground oil storage tank or tanks, together with associated piping and dispensing facilities, located under any land at a single location and used, or intended to be used, for the storage or supply of oil." ;
                      rdfs:label "UNDERGROUND OIL STORAGE FACILITY" .


###  http://sawgraph.spatialai.org/v1/me-egad#siteType.vrap
me_egad:siteType.vrap rdf:type owl:NamedIndividual ,
                               me_egad:EGAD-SiteType ;
                      rdfs:comment "Site where applicants voluntarily investigate and cleanup properties to the DEP's satisfaction, in exchange for protections from DEP enforcement actions." ;
                      rdfs:label "VOLUNTARY RESPONSE ACTION PROGRAM (VRAP)" .


###  http://sawgraph.spatialai.org/v1/me-egad#siteType.wetland
me_egad:siteType.wetland rdf:type owl:NamedIndividual ,
                                  me_egad:EGAD-SiteType ;
                         rdfs:comment "An area inundated or saturated by surface or groundwater where monitoring or assessment activities for quality of water, sediment, habitat, and/or biolgoical communities occur. Includes shallow portions of ponds, lake littoral zones and low gradient strea." ;
                         rdfs:label "WETLAND" .


###  http://sawgraph.spatialai.org/v1/me-egad#siteType.wild-focus-a
me_egad:siteType.wild-focus-a rdf:type owl:NamedIndividual ,
                                       me_egad:EGAD-SiteType ;
                              rdfs:comment "An area used for the collection and assessment of wildlife samples. This can include specific or multiple habitat areas, and can be within either a single town or across multiple towns." ;
                              rdfs:label "WILDLIFE FOCUS AREA" .


###  http://sawgraph.spatialai.org/v1/me-egad#siteType.wood-prod
me_egad:siteType.wood-prod rdf:type owl:NamedIndividual ,
                                    me_egad:EGAD-SiteType ;
                           rdfs:comment "Includes woodyards, wood fuel and woodwaste storage piles associated with power plants, lumberyards, sawmills." ;
                           rdfs:label "WOOD PRODUCTS FACILITY" .


###  Generated by the OWL API (version 4.5.9.2019-02-01T07:24:44Z) https://github.com/owlcs/owlapi
